% no answer key
\documentclass[letterpaper]{exam}

% answer key
% \documentclass[letterpaper, landscape]{exam}
% \usepackage{2in1, lscape} 
% \printanswers

\usepackage{units} 
\usepackage{xfrac} 
\usepackage[fleqn]{amsmath}
\usepackage{float}
\usepackage{mdwlist}
\usepackage{booktabs}
\usepackage{cancel}
\usepackage{polynom}
\usepackage{caption}
\usepackage{fullpage}
\usepackage{comment}
\usepackage{enumerate}
\usepackage{graphicx}

\usepackage{mathtools} 

\newcommand{\dg}{\ensuremath{^\circ}} 
\newcommand{\sgn}{\operatorname{sgn}}

\everymath{\displaystyle}
\title{Calculus I \\ Homework Nine \\ Section 3.1}
\author{}
\date{\today}

\begin{document}

  \maketitle

  \section{Homework}
    \begin{itemize*}
      \item read Section 3.1
      \item exercises: 3-7, 10-15, 20-29, 32-34, 49, 51, 61, 63
    \end{itemize*}

  \ifprintanswers

  \section{Solutions}

  \begin{description}

    \item[3] 
      \[
        f'(x) = \boxed{ 0 } \\
      \]

    \item[4] 
      \[
        f'(x) = \boxed{ 0 } \\
      \]

    \item[5] 
      \[
        f'(t) = \boxed{ - \frac{2}{3} } \\
      \]

    \item[6] 
      \[
        f'(x) = \boxed{ 6 x^7 } \\
      \]

    \item[7] 
      \[
        f'(x) = \boxed{ 3x^2 - 4 } \\
      \]

    % \item[8] 
    %   \[
    %     f'(t) = \boxed{ 3t^5 - 12t^3 + 1 } \\
    %   \]

    % \item[9] 
    %   \[
    %     f'(t) = \boxed{ t^3 } \\
    %   \]

    \item[10] 
      \[
        f'(x) = \boxed{ 4x - 1 } \\
      \]

    \item[11] 
      \[
        y' = \boxed{ -\frac{2}{x^{7/5}} } \\
      \]

    \item[12] 
      \[
        y' = \boxed{ 5e^x } \\
      \]

    \item[13] 
      \[
        V'(r) = \boxed{ 4 \pi r^2 } \\
      \]

    \item[14] 
      \[
        V'(r) = \boxed{ -\frac{3}{x^{8/5}} } \\
      \]

    \item[15] 
      \[
        A'(s) = \boxed{ 60 s^{-6} } \\
      \]

    % \item[16] 
    %   \[
    %     B'(y) = \boxed{ -6 c y^{-7} } \\
    %   \]

    % \item[17] 
    %   \[
    %     G'(x) = \boxed{ \frac{1}{2 \sqrt{x}}-2 e^x } \\
    %   \]

    % \item[18] 
    %   \[
    %     y' = \boxed{ \frac{1}{3} x^{-2/3} } \\
    %   \]

    % \item[19] 
    %   \[
    %     F'(x) = \boxed{ \frac{5}{32} x^4 } \\
    %   \]

    \item[20] 
      \[
        f'(t) = \boxed{ \frac{1}{2 \sqrt{x} + \frac{1}{2 x^{3/2}} } } \\
      \]

    \item[21] 
      \[
        y' = \boxed{ 2ax + b } \\
      \]

    \item[22] 
      \[
        y' = \boxed{ \frac{3 \sqrt{x}}{2}-\frac{1}{2 \sqrt{x}} } \\
      \]

    \item[23] 
      \begin{align*}
        y  & = x^{3/2} - 4x^{1/2} + 3x^{-1/2} \\
        y' & = \boxed{ \frac{3}{2}x^{1/2} + 2x^{-1/2} - \frac{3}{2} x^{-3/2} } \\
      \end{align*}

    \item[24] 
      \begin{align*}
        y  & = x^{3/2} - 2x^{-1/2} \\
        y' & = \boxed{ \frac{3}{2}x^{1/2} + x^{-3/2} } \\
      \end{align*}

    \item[25] 
      \begin{align*}
        y' & = \boxed{ 0 } \\
      \end{align*}

    \item[26] 
      \begin{align*}
        y  & = \sqrt{2} u + \sqrt{3} u^{1/2} \\
        y' & = \boxed{\sqrt{2} + \frac{\sqrt{3}}{2} u^{-1/2}} \\
      \end{align*}

    \item[27] 
      \begin{align*}
        y  & = \left(x + x^{-1} \right)^3 \\
           & = x^3 + x^{-3} + 3x + 3x^{-1} \\
        y' & = \boxed{ 3x^2 - 3x^{-4} + 3 - 3x^{-2} } \\
      \end{align*}

    \item[28] 
      \begin{align*}
        y  & = ae^v + bv^{-1} + cv^{-2} \\
        y' & = \boxed{ ae^v - bv^{-2} - 2cv^{-3} } \\
      \end{align*}

    \item[29] 
      \begin{align*}
        y  & = t^{1/5} + 4t^{5/2} \\
        y' & = \boxed{ \frac{1}{5} t^{-4/5} + 10 t^{3/2} } \\
      \end{align*}

    % \item[30] 
    %   \begin{align*}
    %     v  & = \left( x^{1/2} + x^{-1/3} \right) \\
    %        & = x^{-2/3} + 2x^{1/6} + x \\
    %     v' & = \boxed{ \frac{1}{3 x^{5/6}} - \frac{2}{3 x^{5/3}} + 1 } \\
    %   \end{align*}

    % \item[31] 
    %   \begin{align*}
    %     z  & = Ay^{-10} + Be^y \\
    %     y' & = \boxed{ -10 Ay^{-11} + Be^y } \\
    %   \end{align*}

    \item[32] 
      \begin{align*}
        y  & = e^{x + 1} + 1 \\
           & = e \cdot e^x + 1 \\
        \\
        y' & = e e^x \\
           & = \boxed{ e^{x + 1} } \\
      \end{align*}

    \item[33] 
      find the slope: 
      \begin{align*}
        y     & = x^{1/4} \\
        y'    & = \frac{1}{4} x^{-3/4} \\
        y'(1) & = \frac{1}{4} \\
      \end{align*}

      find the equation:
      \begin{align*}
        \frac{1}{4} & = \frac{y - 1}{x - 1} \\
        y           & = \boxed{ \frac{x}{4} + \frac{3}{4} } \\
      \end{align*}

    \item[34] 
      find the slope: 
      \begin{align*}
        y     & = x^4 - 2x^2 - x \\
        y'    & = 4x^3 - 4x - 1 \\
        y'(1) & = -1 \\
      \end{align*}

      find the equation:
      \begin{align*}
        -1 & = \frac{y - 1}{x - 1} \\
        y  & = \boxed{ -x + 2 } \\
      \end{align*}
      
    \item[49]
      \begin{enumerate}[(a)]
        \item 
          \begin{align*}
            s(t) &= t^3 - 3t \\
            v(t) &= 3t^2 - 3 \\
            a(t) &= 6t \\
          \end{align*}

        \item $a(2) = \boxed{ \unit[12]{m/s^2} }$

        \item
          \begin{align*}
            3t^2 - 3 & = 0 \\
            t        & = \boxed{ \unit[1]{s} } \\
            \\
            a(1)     & = \boxed{ \unit[6]{m/s^2} } \\
          \end{align*}

      \end{enumerate}

    \item[51]
      \begin{align*}
        y              & = 2x^3 + 3x^2 - 12x + 1 \\
        y'             & = 6x^2 + 6x - 12 \\
        \\
        6x^2 + 6x - 12 & = 0 \\
        x              & = \{ -2, 1 \} \\
      \end{align*}

      The points are: \fbox{ $(-2, 21)$ and $(1, -6)$ }.

    \item[61]
      \begin{align*}
        \lim_{h \to 0} \frac{\cfrac{1}{x + h} - \cfrac{1}{x}}{h} & = \lim_{h \to 0} \frac{x - (x + h)}{hx(x + h)} \\
                                                                 & = \lim_{h \to 0} \frac{-h}{hx(x + h)} \\
                                                                 & = - \frac{1}{x^2} \\
      \end{align*}

    \item[63]
      \begin{align*}
        f(x)          & = ax^2 + bx + c \\
        f'(x)         & = 2ax + b \\
        f''(x)        & = 2a \\
        \\
        2a            & = 2 \\
        a             & = 1 \\
        f''(x)        &= 2 \\
        \\
        f'(x)         & = 2x + b \\
        2 \cdot 2 + b & = 3 \\
        b             & = -1 \\
        f'(x)         & = 2x - 1 \\
        \\
        f(x)          & = x^2 - x + c \\
        2^2 - 2 + c   & = 5 \\
        c             & = 3 \\
        \\
        f(x)          & = \boxed{ x^2 - x + 3 } \\
      \end{align*}
   \end{description}
 
  \else
    \vspace{10 cm}
    \begin{quote}
      \begin{em}
        Jail is big business, believe me. I'm in jail, I see the big business.
        You can feed a whole town off one jail. This jail is in the middle of a
        town that feeds everybody. Everybody works here, this is the main
        income. So if there were no criminals, nobody would work.
      \end{em}
    \end{quote}
    \hspace{2 cm} --Tupac Shakur
  \fi

\end{document}

