\documentclass[letterpaper, landscape]{exam}
\usepackage{2in1, lscape} 
\printanswers

\usepackage{units} 
\usepackage[fleqn]{amsmath}
\usepackage{float}
\usepackage{mdwlist}
\usepackage{booktabs}
\usepackage{caption}
\usepackage{fullpage}
\usepackage{enumerate}
\usepackage{graphicx}
\usepackage[justification=justified]{caption}

\setcounter{tocdepth}{1}
\everymath{\displaystyle}

\author{}
\date{\today}
\title{Calculus I \\ Exponentials}

\begin{document}

  \maketitle
  \tableofcontents

  \section{Interest}

  \subsection{Simple Interest} % (fold)
  \[
    A = P + Prt
  \]

  \$1,000 at 5\% interest for 10 years is:
  \[
    A = 1000 + 1000 \cdot 0.05 \cdot 10 = \$1,500
  \]

  \subsection{Compound Interest} % (fold)

  \subsubsection{Compound Yearly} % (fold)
  \begin{align*}
    A_0 &= P + Pr &= P(1 + r) \\
    A_1 &= A_0 + A_0 r &= A_0 (1 + r) = P(1 + r)^2 \\
    A_2 &= A_1 + A_1 r &= A_1 (1 + r) = P(1 + r)^3 \\
    \vdots \\
    A(t) &= P(1 + r)^t \\
  \end{align*}
  
  \$1,000 at 5\% interest for 10 years is:
  \[
    A = 1,000 \cdot (1 + 0.05)^{10} = \$1,628.89
  \]

  \subsubsection{Compounded More Frequently} % (fold)

  $n$ compoundings per year
  \begin{align*}
    A(t) &= P \left(1 + \frac{r}{n} \right)^nt
  \end{align*}
  
  Compounded monthly
  \[
    A = 1,000 \cdot \left( 1 + \frac{0.05}{12} \right)^{10 \cdot 12} = \$1,647.01
  \]

  Compounded daily
  \[
    A = 1,000 \cdot \left( 1 + \frac{0.05}{8760} \right)^{10 \cdot 8760} = \$1,648.66
  \]

  Compounded hourly
  \[
    A = 1,000 \cdot \left( 1 + \frac{0.05}{8760} \right)^{10 \cdot 8760} = \$1,648.72
  \]

  \subsection{Continuous Compounding} % (fold)
  
  \begin{align*}
    A    & = \lim_{n \to \infty} A \left( 1 + \frac{r}{n} \right)^{nt}
    \\
    x    & = \frac{r}{n} \
    \\
    A    & = \lim_{x \to 0} A \left( 1 + x \right)^{rt/x} \\
         & = \lim_{x \to 0} A \left[ \left( 1 + x \right)^{1/x} \right]^{rt} \\
    \\
    e    & = \lim_{x \to 0} \left( 1 + x \right)^{1/x} \\
    \\
    A(t) & = P e^{rt} \\
  \end{align*}


  \section{Calculating e} % (fold)
  
  Draw Pascal's Triangle.

  \begin{align*}
    (a & + b)^n = a^n + a^{n - 1} b \cdot \frac{n}{1!} + a^{n - 2} b^2 \cdot \frac{n(n - 1)}{2!} \\
       &+ a^{n - 3} b^3 \cdot \frac{n(n - 1)(n - 2)}{3!} + \ldots + b^n
    \left[ (1 + n)^{1/n} \right]^n &= 
  \end{align*}

  \begin{align*}
    e &= \lim_{n \to \infty} \left( 1 + \frac{1}{n} \right)^n \\
      & = \lim_{n \to \infty} \left( 1 + \frac{1}{n} \cdot n + \frac{1}{n^2} \cdot \frac{n(n - 1)}{2!} 
        + \frac{1}{n^3} \cdot \frac{n(n - 1)(n - 2)}{3!} + \ldots \right) \\
      & = 1 + 1 + \frac{1}{2!} + \frac{1}{3!} + \frac{1}{4!} + \ldots
    \\
    e^x &= \lim_{n \to \infty} \left( 1 + \frac{1}{n} \right)^{nx} \\
      & = \lim_{n \to \infty} \left( 1 + \frac{1}{n} \cdot nx + \frac{1}{n^2} \cdot \frac{nx(nx - 1)}{2!} 
        + \frac{1}{n^3} \cdot \frac{nx(nx - 1)(nx - 2)}{3!} + \ldots \right) \\
      & = 1 + x + \frac{x^2}{2!} + \frac{x^3}{3!} + \frac{x^4}{4!} + \ldots
    \\
    \frac{d}{dx} e^x &= \frac{d}{dx} \left( 1 + x + \frac{x^2}{2} + \frac{x^3}{3} + \ldots  \right)
  \end{align*}

  \section{Logarithms} % (fold)

  \subsection{History} % (fold)
  
  \begin{itemize*}
    \item Napier turning multiplication into addition, etc.
    \item Tables
  \end{itemize*}
  
  \subsection{Rules} % (fold)
  
  \begin{align*}
    e^x e^y                    & = e^{x + y} \\
    \ln \left( e^x e^y \right) & = \ln e^{x + y} \\
                               & = x + y
    \\
    \ln ab &= \ln a + \ln b \\
  \end{align*}

  \begin{align*}
    \frac{e^x}{e^y}             & = e^{x - y} \\
    \ln \left( e^x e^y \right)  & = \ln e^{x - y} \\
                                & = x - y
    \\
    \ln \frac{a}{b}             & = \ln a - \ln b \\
  \end{align*}

  powers:
  \begin{align*}
    a       & = e^{\ln a} \\
    a^b     & = e^{b \ln a} \\
    \ln a^b & = \ln e^{b \ln a} \\
            & = b \ln a \\
  \end{align*}

  \section{Derivative of $a^x$} % (fold)

  approach one:
  \begin{align*}
    \frac{d}{dx} a^x & = \lim_{h \to 0} \frac{a^{x + h} - a^x}{h} \\
                     & = \lim_{h \to 0} \frac{a^x \left( a^h - 1 \right)}{h} \\
                     & = a^x \lim_{h \to 0} \frac{a^x \left( a^h - 1 \right)}{h} \\
  \end{align*}

  Find $a$ where limit is 1 for simplest result:
  \begin{align*}
    \frac{a^h - 1}{h} & = 1 \\
    a^h - 1           & = h \\
    a^h               & = h + 1 \\
    a                 & = \left( h + 1 \right)^{1/h} \\
    \lim_{h \to 0} a  & = \lim_{h \to 0} \left( h + 1 \right)^{1/h} \\
    a                 & = \lim_{h \to 0} \left( h + 1 \right)^{1/h} \\
    a                 & = e \\
    \frac{d}{dx} e^x  & = e^x \\
  \end{align*}

  approach two:
  \begin{align*}
    \frac{d}{dx} e^x &= \frac{d}{dx} \left( 1 + x + \frac{x^2}{2} + \frac{x^3}{3} + \ldots  \right)
    \ldots
  \end{align*}
  
\end{document}

