% no answer key
% \documentclass[letterpaper]{exam}

% answer key
\documentclass[letterpaper, landscape]{exam}
\usepackage{2in1, lscape} 
\printanswers

\usepackage{units} 
\usepackage{xfrac} 
\usepackage[fleqn]{amsmath}
\usepackage{float}
\usepackage{mdwlist}
\usepackage{booktabs}
\usepackage{cancel}
\usepackage{polynom}
\usepackage{caption}
\usepackage{fullpage}
\usepackage{comment}
\usepackage{enumerate}
\usepackage{graphicx}

\usepackage{mathtools} 

\newcommand{\dg}{\ensuremath{^\circ}} 
\newcommand{\sgn}{\operatorname{sgn}}

\everymath{\displaystyle}
\title{Calculus I \\ Homework Fourteen \\ Section 3.6}
\author{}
\date{\today}

\begin{document}

  \maketitle

  \section{Homework}
    \begin{itemize*}
      \item read Section 3.6
      \item exercises: 2-10, 14-19, 23-26, 31-32, 36-37, 41-42, 45, 49
    \end{itemize*}

  \ifprintanswers

  \section{Solutions}

  \begin{description}

    \item[2] 
      \[
        f'(x) = \boxed{ \frac{2x}{x^2 + 10} }
      \]

    \item[3] 
      \[
        f'(x) = \boxed{ \frac{\cos (\ln x)}{x} }
      \]

    \item[4] 
      \begin{align*}
        f(x) & = \frac{1}{\sin^2 x} \cdot 2 \sin x \cdot \cos x \\
             & = \boxed{ 2 \cot x } \\
      \end{align*}

    \item[5] 
      \[
        f'(x) = \boxed{ \frac{3}{\ln 2 \cdot (3x - 1)} }
      \]

    \item[6] 
      \begin{align*}
        f'(x) & = \frac{1}{\ln 5 \cdot x e^x} \cdot \left( x e^x + e^x \right) \\
              & = \boxed{ \frac{x + 1}{x \log 5} } \\
      \end{align*}

    \item[7] 
      \[
        f'(x) = \boxed{ \frac{1}{5x \ln^{4/5} x} } \\
      \]

    \item[8] 
      \begin{align*}
        f(x)  & = \ln x^{1/5} \\
              & = \frac{1}{5} \ln x \\
        \\
        f'(x) & = \boxed{ \frac{1}{5x} } \\
      \end{align*}

    \item[9] 
      \[
        f'(x) = \boxed{ (\ln 5x + 1) \cos(x \ln 5x ) }
      \]

    \item[10] 
      \begin{align*}
        f'(x) & = \frac{(1 - \ln x) \cdot 1/x - (1 + \ln x) \cdot (-1/x)}{(1 - \ln x)^2} \\
              & = \boxed{ \frac{2}{x (\ln x - 1)^2} } \\
      \end{align*}

    \item[14] 
      \[
        F'(y) = \boxed{ \frac{e^y}{e^y + 1} + \ln \left( e^y + 1 \right) }
      \]

    \item[15] 
      \[
        f'(u) = \boxed{ \frac{1 + \ln 2}{u (\ln 2u + 1)^2} }
      \]

    \item[16] 
      \begin{align*}
        y  & = (\ln x)^{-1} \\
        y' & = - (\ln x)^{-2} \cdot \frac{1}{x} \\
           & = \boxed{ - \frac{1}{x \ln^2 x} } \\
      \end{align*}

    \item[17] 
      \begin{align*}
        y' & = \frac{1}{2 - x - 5x^2} \cdot (-10x - 1) \\
           & = \boxed{ \frac{10x + 1}{5x^2 + x + 2} } \\
      \end{align*}

    \item[18] 
      \begin{align*}
        H(z)  & = \frac{1}{2} \left[ \ln(a^2 - z^2) - \ln(a^2 + z^2)  \right] \\
        H'(z) & = \frac{1}{2} \left[ \frac{-2z}{a^2 - z^2} - \frac{2z}{a^2 + z^2} \right] \\
              & = \boxed{ \frac{2 a^2z^2}{z^4 - a^4} } \\
      \end{align*}

    \item[19] 
      \begin{align*}
        y' & = \frac{1}{e^{-x} + x e^{-x}} \cdot \left[ - e^{-x} - x e^{-x} + e^{-x} \right] \\
           & = \frac{- x e^{-x}}{e^{-x} + x e^{-x}} \\
           & = \boxed{ \frac{ - x}{1 + x} } \\
      \end{align*}

    \item[23] 
      \begin{align*}
        f'(x)  & = \boxed{ x + 2x \ln(2x) } \\
        f''(x) & = \boxed{ 3 + 2 \ln(2x) } \\
      \end{align*}

    \item[24] 
      \begin{align*}
        f'(x)  & = \boxed{ \frac{1 - 2 \ln (x)}{x^3} } \\
        f''(x) & = \boxed{ \frac{6 \ln (x) - 5}{x^4} } \\
      \end{align*}

    \item[25] 
      \begin{align*}
        f'(x)  & = \boxed{ \frac{1}{\sqrt{x^2 + 1}} } \\
        f''(x) & = \boxed{ \frac{x}{ \left( x^2 + 1 \right)^{3/2} } } \\
      \end{align*}

    \item[26] 
      \begin{align*}
        f'(x)  & = \frac{1}{\sec x + \tan x} \cdot (\sec x \tan x + \sec^2 x) \\
               & = \sec x \cdot \frac{\sec x + \tan x}{\sec x + \tan x} \\
               & = \boxed{ \sec x } \\
        f''(x) & = \boxed{ \sec x \tan x } \\
      \end{align*}
      
    \item[31] 
      \begin{align*}
        f'(x) & = \frac{1 - 2 \log x}{x^3} \\
        f'(1) & = \boxed{ 1 } \\
      \end{align*}

    \item[32] 
      \begin{align*}
        f'(x) & = \frac{2 e^{2x}}{e^{2x} + 1} \\
        f'(0) & = \boxed{ 1 } \\
      \end{align*}

    \item[36] 
      \begin{align*}
        y            & = (2x + 1)^5 \left( x^4 - 3 \right)^6 \\
        \ln y        & = 5 \ln (2x + 1) + 6 \ln \left( x^4 - 3 \right) \\
        \frac{y'}{y} & = \frac{10}{2x + 1} + \frac{24x^3}{x^4 - 3} \\
        y'           & = (2x + 1)^5 \left(x^4 - 3\right)^6 \left( \frac{10}{2x + 1} + \frac{24x^3}{x^4 - 3} \right) \\
                     & = \boxed{ 10 (2x + 1)^4 \left( x^4 - 3 \right)^6 + 24x^3 (2x + 1)^5 \left( x^4 - 3 \right)^5 } \\
      \end{align*}
      
    \item[37] 
      \begin{align*}
        y            & = x^{1/2} e^{x^2} \left( x^2 + 1 \right)^{10} \\
        \ln y        & = \frac{1}{2} \ln x + x^2 + 10 \ln \left( x^2 + 1 \right) \\
        \frac{y'}{y} & = \frac{1}{2x} + 2x + \frac{20x}{x^2 + 1} \\
        y'           & = \boxed{ x^{1/2} e^{x^2} \left( x^2 + 1 \right)^{10} \left( \frac{1}{2x} + 2x + \frac{20x}{x^2 + 1} \right) } \\
                     % & = \boxed{ \frac{e^{x^2} \left(x^2 + 1\right)^{10}}{2 \sqrt{x}} + 2 e^{x^2} 
                     %             \left(x^2 + 1\right)^{10} x^{3/2} + 20 e^{x^2} \left(x^2 + 1\right)^9x^{3/2} }      
      \end{align*}

    \item[41] 
      \begin{align*}
        y            & = x^x \\
        \ln y        & = x \ln x \\
        \frac{y'}{y} & = 1 + \ln x \\
        y'           & = \boxed{ x^x (1 + \ln x) } \\
      \end{align*}

    \item[42] 
      \begin{align*}
        y            & = x^{\cos x} \\
        \ln y        & = \cos x \ln x \\
        \frac{y'}{y} & = \frac{\cos x}{x} - \sin x \ln x \\
        y'           & = \boxed{ x^{\cos x} \left( \frac{\cos x}{x} - \sin x \ln x \right) } \\
      \end{align*}

    \item[45] 
      \begin{align*}
        y            & = (\cos x)^x \\
        \ln y        & = x \ln (\cos x) \\
        \frac{y'}{y} & = - \frac{x \sin x}{\cos x} + \ln (\cos x) \\
        y'           & = \boxed{ (\cos x)^x (\ln (\cos x) - x \tan x) } \\
      \end{align*}

    \item[49] 
      \begin{align*}
        y  & = \ln \left( x^2 + y^2 \right) \\
        y' & = \frac{2x + 2yy'}{x^2 + y^2} \\
           & = \boxed{ \frac{2x}{x^2 + y^2 - 2 y} } \\
      \end{align*}

    % \item[50] 
    %   \begin{align*}
    %     x^y &= y^x \\
    %     y \ln x &= x \ln y \\
    %     \frac{y}{x} + y' \ln x &= \frac{x}{y y'} + \ln y \\
    %   \end{align*}
  \end{description}

  \else
    \vspace{10 cm}
    \begin{quote}
      \begin{em}
        Real ``change that you could believe in'' would be an end to empire,
        and an end to wars for corporate greed, not just a change of the shade
        of the political managers.
      \end{em}
    \end{quote}
    \hspace{2 cm} --Mumia Abu-Jamal
  \fi

\end{document}

