
\documentclass[fleqn,addpoints]{exam}

\usepackage{amsmath}
\usepackage{graphics}
\usepackage{cancel}
\usepackage{polynom}
\usepackage{mdwlist}

\printanswers

\ifprintanswers
\usepackage{2in1, lscape}
\fi

\title{Math 113 Homework 12}
\author{}
\date{\today}

\begin{document}

\maketitle

\section{From the Book}

Read pages 245-263.

\begin{itemize*}
  \item pp. 249-251: 11-12, 19-20, 40-44, 58-59, 70-74, 77
  \item pp. 256-257: 20-24, 40-44, 51, 52, 65-69
\end{itemize*}

% 175 points possible

\section{Additional Problems}

The ratio of the width of the {\em Temple of Hephaestus} to its height is approximately
\[
  \dfrac{w}{h} = \dfrac{2}{\sqrt{5} - 1}
\]

This number is called the {\em golden section}.  Early Greeks believed that the most aesthetically pleasing rectangles
were those whose sides had this ratio.  Rationalize the denominator for this expression.

\begin{solution}
\[
  \frac{2}{\sqrt{5} - 1} \left( \frac{\sqrt{5} + 1}{\sqrt{5} + 1} \right) = \frac{2(\sqrt{5} + 1)}{5-1} = \frac{\sqrt{5} + 1}{2}
\]

\end{solution}

\section{Extra Credit}

Two ferryboats start at the same instant from opposite sides of a river, traveling across the water on routes at right
angles to the shores.  Each travels at a constant speed, but one is faster than the other.  They pass at a point 720
yards from the nearest shore.  Both boats remain at the dock for 10 minutes before starting back.  On the return trips,
they meet 400 yards from the other shore.

How wide is the river?

\begin{solution}

Let $x$ be the length of the river. The exact time spent at the dock doesn't matter---the important point is that the two
boats spend the same time at their docks.  There are two meeting times mentioned in the problem statement.  

The first time the boats meet, the slow boat has traveled 720 yards from shore and the fast boat has traveled $x-720$ yards
from the other shore.  We know that the slow boat is the one that is 720 yards from shore because they pass at a point
720 yards from the {\em nearest} shore and the fast boat will have gone farther than the slow boat when they meet.

The second time the boats meet, the slow boat has reached the opposite shore and traveled 400 yards back on the return trip.  The fast boat
is 400 yards away from completing its round trip.  So at the second meeting, the slow boat has traveled $x+400$ yards and
the fast boat has traveled $2x-400$ yards.

Now we need a single equation that includes $x$.  Since the boats are traveling at constant rates, the ratios of the
distances each boat has traveled must be constant.  You can see this from:

\[
   \frac{d_{slow}}{d_{fast}} = \frac{r_{slow}\cancel{t}}{r_{fast} \cancel{t}} = \frac{r_{slow}}{r_{fast}}
\]

Since the rates don't change, $\dfrac{r_{slow}}{r_{fast}}$ is constant and the ratios of the distances at any particular
time will also be constant.  

We can now set up an equation using the ratios of the distances at the two times:
\begin{align*}
  \frac{x+400}{2x-400} &= \frac{720}{x-720} \\
  (x+400)(x-720) &= 720(2x-400) \\
  x^2-1760x &= 0 \\
  x(x-1760) &= 0 
\end{align*}

$x = \{0, 1760\}$, but 0 doesn't make sense for this problem and 1,760 yards is the width of the river.

\end{solution}

\ifprintanswers

\section{Pages 249-251}

\begin{description}

\item[11]
\[
  \frac{3}{4}\sqrt{7} - \frac{2}{3}\sqrt{28} = \frac{3}{4}\sqrt{7} - \frac{2}{3}\sqrt{4 \cdot 7} 
  = \frac{3}{4}\sqrt{7} - \frac{4}{3}\sqrt{7}  = \frac{-7\sqrt{7}}{12}
\]

\item[12]
\[
  \frac{3}{5}\sqrt{5} - \frac{1}{4}\sqrt{80} = \frac{3}{5}\sqrt{5} - \frac{1}{4}\sqrt{16 \cdot 4}
  = \frac{3}{5}\sqrt{5} - \sqrt{5} = \frac{-2\sqrt{5}}{5}
\]

% \item[13]
% \begin{align*}
%   \frac{3}{5}\sqrt{40} + \frac{5}{6}\sqrt{90} &= \frac{3}{5}\sqrt{4 \cdot 10} + \frac{5}{6}\sqrt{9 \cdot 10} \\
%   &= \frac{6}{5}\sqrt{10} + \frac{15}{6}\sqrt{10} \\
%   &= \frac{6}{5}\sqrt{10} + \frac{5}{2}\sqrt{10} \\
%   &= \frac{37\sqrt{10}}{10} \\
% \end{align*}

% \item[14]
% \[
%   \frac{3}{8}\sqrt{96} - \frac{2}{3}\sqrt{54} = \frac{3}{8}\sqrt{16 \cdot 6} - \frac{2}{3}\sqrt{9 \cdot 6}
%   = \frac{12}{8}\sqrt{6} - \frac{6}{3}\sqrt{6} = \frac{-5\sqrt{6}}{4}
% \]

\item[19]
\begin{align*}
  & -\sqrt[3]{16} +7\sqrt[3]{54} - 9\sqrt[3]{2} = -\sqrt[3]{8 \cdot 2} +7\sqrt[3]{27 \cdot 2} - 9\sqrt[3]{2} \\
  &= -2\sqrt[3]{2} + 21\sqrt[3]{2} - 9\sqrt[3]{2} = 10\sqrt[3]{2}
\end{align*}

\item[20]
\begin{align*}
  & 4\sqrt[3]{24} - 6\sqrt[3]{3} + 13\sqrt[3]{81} = 4\sqrt[3]{8 \cdot 3} - 6\sqrt[3]{3} + 13\sqrt[3]{27 \cdot 3} \\
  &= 8\sqrt[3]{3} - 6\sqrt[3]{3} + 39\sqrt[3]{3} = 41\sqrt[3]{3}
\end{align*}

\item[40]
\[
  \sqrt{\frac{7}{8x^2}} = \frac{\sqrt{7}}{\sqrt{2 \cdot 4x^2}} 
  = \frac{\sqrt{7}}{2x\sqrt{2}} \left( \frac{\sqrt{2}}{\sqrt{2}} \right) = \frac{\sqrt{14}}{4x}
\]

\item[41]
\[
  \frac{5}{\sqrt{18y}} = \frac{5}{3\sqrt{2y}} \left( \frac{\sqrt{2y}}{\sqrt{2y}} \right) = \frac{5\sqrt{2y}}{6y}
\]

\item[42]
\[
  \frac{3}{\sqrt{12x}} = \frac{3}{2\sqrt{3x}} \left( \frac{\sqrt{3x}}{\sqrt{3x}} \right) = \frac{3\sqrt{3x}}{6x} = \frac{\sqrt{3x}}{2x}
\]

\item[43]
\[
  \frac{\sqrt{7x}}{\sqrt{8y^5}} = \frac{\sqrt{7x}}{2y^2\sqrt{2y}} \left( \frac{\sqrt{2y}}{\sqrt{2y}} \right) 
  = \frac{\sqrt{14xy}}{4y^3}
\]

\item[44]
\[
  \frac{\sqrt{5y}}{\sqrt{18x^3}} = \frac{\sqrt{5y}}{3x\sqrt{2x}} \left( \frac{\sqrt{2x}}{\sqrt{2x}} \right) 
  = \frac{\sqrt{10xy}}{6x^2}
\]

% \item[55]
% \[
%   \sqrt[3]{\frac{7}{9x^2}} = \frac{\sqrt[3]{7}}{\sqrt[3]{9x^2}} 
%   = \frac{\sqrt[3]{7}}{\sqrt[3]{3^2x^2}} \left( \frac{\sqrt[3]{3x}}{\sqrt[3]{3x}} \right)
%   = \frac{\sqrt[3]{21x}}{3x}
% \]

% \item[56]
% \[
%   \sqrt[3]{\frac{5}{2x}} = \frac{\sqrt[3]{5}}{\sqrt[3]{2x}} \left( \frac{\sqrt[3]{2^2x^2}}{\sqrt[3]{2^2x^2}} \right)
%   = \frac{\sqrt[3]{20x^2}}{\sqrt[3]{2^3x^3}} = \frac{\sqrt[3]{20x^2}}{3x}
% \]

% \item[57]
% \[
%   \frac{\sqrt[3]{3y}}{\sqrt[3]{16x^4}} 
%   = \frac{\sqrt[3]{3y}}{2x\sqrt[3]{2x}} \left( \frac{\sqrt[3]{2^2x^2}}{\sqrt[3]{2^2x^2}} \right)
%   = \frac{\sqrt[3]{12x^2y}}{2\sqrt[3]{2^3x^3}} = \frac{\sqrt[3]{12x^2y}}{4x} 
% \]

\item[58]
\[
  \frac{\sqrt[3]{2y}}{\sqrt[3]{3x}} \left( \frac{\sqrt[3]{3^2x^2}}{\sqrt[3]{3^2x^2}} \right) 
  = \frac{\sqrt[3]{18x^2y}}{3x}
\]

\item[59]
\begin{align*}
  \frac{\sqrt[3]{12xy}}{\sqrt[3]{3x^2y^5}} &= \frac{\sqrt[3]{12xy}}{y\sqrt[3]{3x^2y^2}}
     \left(\frac{\sqrt[3]{3^2xy}}{\sqrt[3]{3^2xy}} \right) \\
  &= \frac{\sqrt[3]{3^32^2x^2y^2}}{3xy^2} \\
  &= \frac{\cancel{3} \sqrt[3]{4x^2y^2}}{\cancel{3}xy^2} \\
  &= \frac{\sqrt[3]{4x^2y^2}}{xy^2}
\end{align*}

% \item[60]
% \[
%   \frac{5}{\sqrt[3]{9xy^2}} = \frac{5}{\sqrt[3]{3^2xy^2}} \left( \frac{\sqrt[3]{3x^2y}}{\sqrt[3]{3x^2y}} \right)
%   = \frac{5\sqrt[3]{3x^2y}}{3xy}
% \]

\item[70]
\[
  4\sqrt{8n} + 3\sqrt{18n} - 2\sqrt{72n} = 8\sqrt{2n} + 9\sqrt{2n} - 12\sqrt{2n} = 5\sqrt{2n}
\]

\item[71]
\[
  7\sqrt{4ab} - \sqrt{16ab} - 10\sqrt{25ab} = 14\sqrt{ab} - 4\sqrt{ab} - 50\sqrt{ab} = -40\sqrt{ab}
\]

\item[72]
\[
  4\sqrt{ab} - 9\sqrt{36ab} + 6\sqrt{49ab} = 4\sqrt{ab} - 54 \sqrt{ab} + 42\sqrt{ab} = -8\sqrt{ab}
\]

\item[73]
\begin{align*}
  & -3\sqrt{2x^3} + 4\sqrt{8x^3} - 3\sqrt{32x^3} = -3x\sqrt{2x} + 8x\sqrt{2x} - 12x\sqrt{2x} \\
  &= -7x\sqrt{2x}
\end{align*}

\item[74]
\begin{align*}
  & 2\sqrt{40x^5} - 3\sqrt{90x^5} + 5\sqrt{160x^5} \\
  &= 4x^2\sqrt{10x} - 9x^2\sqrt{10x} + 20x^2\sqrt{10x} \\
  &= 15x^2\sqrt{10x}
\end{align*}

\item[77]
\begin{align*}
  (\sqrt{x+y})^2 &= x + y \\
  (\sqrt{x} + \sqrt{y})^2 &= x + 2\sqrt{xy} + y
\end{align*}

\end{description}

\section{Pages 256-257}

\begin{description}
\item[20]
\[
  4\sqrt{2}(3\sqrt{12} + 7\sqrt{6}) = 24\sqrt{6} + 56\sqrt{3}
\]

\item[21]
\begin{align*}
  & -4\sqrt{5}(2\sqrt{5} + 4\sqrt{12}) \\
  &= -4\sqrt{5}(2\sqrt{5} + 8\sqrt{3}) \\
  &= -8 \cdot 5 - 32\sqrt{15} = -40 - 32\sqrt{15}
\end{align*}

\item[22]
\[
  -5\sqrt{3}(3\sqrt{12} - 9\sqrt{8}) = -5\sqrt{3}(6\sqrt{3} - 18\sqrt{2}) = -90 + 90\sqrt{6}
\]

\item[23]
\[
  3\sqrt{x}(5\sqrt{2} + \sqrt{y}) = 15\sqrt{2x} + 3\sqrt{xy}
\]

\item[24]
\[
  \sqrt{2x}(3\sqrt{y} - 7\sqrt{5}) = 3\sqrt{2xy} - 7\sqrt{10x}
\]

\item[40]
\[
  (7\sqrt{3} - \sqrt{7})(2\sqrt{3} + 4\sqrt{7}) = 14 \cdot 3 + 28\sqrt{21} - 7 \cdot 2 \sqrt{21} - 28 = 14 + 26 \sqrt{21}
\]

\item[41]
\[
 (3\sqrt{2} - 5\sqrt{3})(6\sqrt{2} - 7\sqrt{3}) = 18 \cdot 2 - 21\sqrt{6} - 30\sqrt{6} + 35 \cdot 3 = 141 - 51\sqrt{6}
\]

\item[42]
\begin{align*}
  & (\sqrt{8} - 3\sqrt{10})(2\sqrt{8} - 6\sqrt{10}) = 16 - 6\sqrt{80} - 6\sqrt{80} + 18 \cdot 10 \\
  &= 16 - 12\sqrt{80} + 180 = 196 -48\sqrt{5}
\end{align*}

\item[43]
\[
  (\sqrt{6} + 4)(\sqrt{6} - 4) = 6 - 16 = -10
\]

\item[44]
\[
  (\sqrt{7} + 2)(\sqrt{7} - 2) = 7 - 4 = 3
\]

\item[51]
\[
  3\sqrt[3]{4}(2\sqrt[3]{2} - 6\sqrt[3]{4}) = 6\sqrt[3]{8} - 18\sqrt[3]{16} = 12 - 36\sqrt[3]{2}
\]

\item[52]
\[
  3\sqrt[3]{3}(4\sqrt[3]{9} + 5\sqrt[3]{7}) = 12\sqrt[3]{27} + 15\sqrt[3]{21} = 36 + 15\sqrt[3]{21}
\]

\item[65]
\begin{align*}
  & \frac{\sqrt{6}}{3\sqrt{2} + 2\sqrt{3}} \left( \frac{{3\sqrt{2} - 2\sqrt{3}}}{{3\sqrt{2} - 2\sqrt{3}}} \right) \\
  &= \frac{3\sqrt{12} - 2\sqrt{18}}{9 \cdot 2 - 4 \cdot 3} \\
  &= \frac{6\sqrt{3} - 6\sqrt{2}}{6} \\
  &= \frac{\cancel{6} (\sqrt{3} - \sqrt{2})}{\cancel{6}} \\
  &= \sqrt{3} - \sqrt{2} \\
\end{align*}

\item[66]
\[
  \frac{3\sqrt{6}}{5\sqrt{3} - 4\sqrt{2}} \left( \frac{5\sqrt{3} + 4\sqrt{2}  }{5\sqrt{3} + 4\sqrt{2}} \right) 
  = \frac{15\sqrt{18} + 12\sqrt{12}}{75 - 32} = \frac{45\sqrt{2} + 24\sqrt{3}}{43}
\]

\item[67]
\[
  \frac{2}{\sqrt{x} + 4} \left( \frac{\sqrt{x} - 4}{\sqrt{x} - 4} \right) = \frac{2\sqrt{x} - 8}{x-16}
\]

\item[68]
\[
  \frac{3}{\sqrt{x} + 7} \left( \frac{\sqrt{x} - 7}{\sqrt{x} - 7} \right) = \frac{3\sqrt{x} - 21}{x-49}
\]

\item[69]
\[
  \frac{\sqrt{x}}{\sqrt{x} - 5} \left( \frac{\sqrt{x} + 5}{\sqrt{x} + 5} \right) = \frac{x + 5\sqrt{x}}{x-25}
\]

\end{description}

\else
\vspace{3 cm}

{\em
\begin{verse}
now is a ship

which captain am \\
sails out of sleep 

steering for dream 
\end{verse}
}

\hspace{1 in} e.e. cummings

\fi

\end{document}

\end{document}
