% no answer key
% \documentclass[letterpaper]{exam}

% answer key
\documentclass[letterpaper, landscape]{exam}
\usepackage{2in1, lscape} 
\printanswers

\usepackage{units} 
\usepackage{xfrac} 
\usepackage[fleqn]{amsmath}
\usepackage{cancel}
\usepackage{float}
\usepackage{mdwlist}
\usepackage{booktabs}
\usepackage{cancel}
\usepackage{polynom}
\usepackage{caption}
\usepackage{fullpage}
\usepackage{comment}
\usepackage{enumerate}
\usepackage{graphicx}

\newcommand{\dg}{\ensuremath{^\circ}} 
\everymath{\displaystyle}

\title{Calculus I \\ Homework Three \\ Section 2.3}
\author{}
\date{\today}

\begin{document}

  \maketitle

  \section{Homework}
    \begin{itemize*}
      \item read Section 2.3
      \item exercises: TO DO
    \end{itemize*}

  \ifprintanswers

    \section{Solutions}

    \begin{description}

      \item[1]
        \begin{enumerate}[(a)]
          \item $\lim_{x \to 2} \left[ f(x) + 5g(x) \right] = \boxed{ -6 }$
          \item $\lim_{x \to 2} \left[ g(x) \right]^3 = \boxed{ -8 }$
          \item $\lim_{x \to 2} \sqrt{f(x)} = \boxed{ 2 }$
          \item $\lim_{x \to 2} \frac{3 f(x)}{g(x)} = \boxed{ -6 }$
          \item $\lim_{x \to 2} \frac{g(x) h(x)}{f(x)} \boxed{ 0 }$ 
        \end{enumerate}

      \item[2]
        \begin{enumerate}[(a)]
          \item $\lim_{x \to 2} \left[ f(x) + g(x) \right] = \boxed{ 2 }$
          \item $\lim_{x \to 1} \left[ f(x) + g(x) \right]$ does not exist 
          \item $\lim_{x \to 0} \left[ f(x) g(x) \right] = \boxed{ 0 } $ 
          \item $\lim_{x \to -1} \left[ \frac{f(x)}{g(x)} \right]$ does not exist
          \item $\lim_{x \to 2} \left[ x^3 f(x) \right] = \boxed{ 16 } $ 
          \item $\lim_{x \to 1} \sqrt{3 + f(x)} = \boxed{ 4 }$ 
        \end{enumerate}

      \item[3]
        \[
          \lim_{x \to -2} \left( 3x^4 + 2x^2 - x + 1 \right) = \boxed{ 59 }
        \]

      \item[4]
        \[
          \lim_{x \to 2} \left( \frac{2x^2 + 1}{x^2 + 6x - 4} \right) 
              = \boxed{ \frac{3}{4} }
        \]

      \item[8]
        \[
          \lim_{u \to -2} \sqrt{ u^4 + 3u + 6} = \boxed{ 2 \sqrt{7} }
        \]

      \item[9]
        \[
          \lim_{x \to 4^-} \sqrt{ 16 - x^2 } = \boxed{ 0 }
        \]

      \item[10]
        \begin{enumerate}[(a)]
          \item $f(2)$ is not defined on the left side and is defined on the
            right side

          \item It doesn't matter whether $f(2)$ is defined when determining the
            limit.
        \end{enumerate}

      \item[11]
        \[
          \lim_{x \to 2} \frac{x^2 + x - 6}{x - 2} 
            = \lim_{x \to 2} (x + 3) = \boxed{ 5 } 
        \]

      \item[12]
        \[
          \lim_{x \to -4} \frac{x^2+5 x+4}{x^2+3 x-4} 
            = \lim_{x \to -4} \frac{x+1}{x-1} = \boxed{ \frac{3}{5} } 
        \]

      \item[15]
        \[
          \lim_{t \to -3} \frac{t^2-9}{2 t^2+7 t+3}            
            = \lim_{t \to -3} \frac{t-3}{2 t+1} = \boxed{ \frac{6}{5} } 
        \]

      \item[16]
        \[
          \lim_{x \to -1} \frac{x^2-4 x}{x^2-3 x-4} 
            = \lim_{x \to -1} \frac{x}{x+1} = \boxed{ -\infty } 
        \]

      \item[17]
        \[
          \lim_{x \to 0} \frac{(x+4)^2-16}{x} 
            = \lim_{x \to 0} x + 8 = \boxed{ 8 } 
        \]

      \item[18]
        \[
          \lim_{x \to 1} \frac{x^3-1}{x^2-1} 
            = \lim_{x \to 1} \frac{x^2+x+1}{x+1} = \boxed{ \frac{3}{2} } 
        \]

      \item[19]
        \[
          \lim_{x \to -2} \frac{x+2}{x^3+8} 
            = \lim_{x \to -2} \frac{1}{x^2-2 x+4} = \boxed{ \frac{1}{12} } 
        \]

      \item[20]
        \[
          \lim_{x \to 0} \frac{(x+2)^3-8}{x} 
            = \lim_{x \to 0} x^2+6 x+12 = \boxed{ 12 } 
        \]

      \item[21]
        \[
          \lim_{x \to 9} \frac{9-x}{3-\sqrt{x}} 
            = \lim_{x \to 9} \sqrt{x}+3 = \boxed{ 6 } 
        \]

      \item[22]
        \[
          \lim_{x \to 0} \frac{\sqrt{x+1}-1}{x} 
            = \lim_{x \to 0} \frac{1}{\sqrt{x + 1} + 1} 
            = \boxed{ \frac{1}{2} } 
        \]

      \item[23]
        \[
          \lim_{x \to 7} \frac{\sqrt{x+2}-3}{x-7} 
            = \lim_{x \to 7} \frac{1}{\sqrt{x + 2} + 3} 
            = \boxed{ \frac{1}{6} } 
        \]

      \item[24]
        \[
          \lim_{x \to -1} \frac{x^2+2 x+1}{x^4-1} 
            = \lim_{x \to -1} \frac{x+1}{(x^2+1)(x-1)} 
            = \boxed{ 0 } 
        \]

      \item[25]
        \[
          \lim_{x \to -4} \frac{\sfrac{1}{x}+\sfrac{1}{4}}{x+4} 
            = \lim_{x \to -4} \frac{1}{4 x} 
            = \boxed{ -\frac{1}{16} } 
        \]

      \item[26]
        \[
          \lim_{t \to 0} \frac{1}{t}-\frac{1}{t^2+t} 
            = \lim_{t \to 0} \frac{1}{t + 1} 
            = \boxed{ 1 } 
        \]

      \item[27]
        \[
          \lim_{x \to 16} \frac{4-\sqrt{x}}{16 x-x^2} 
            = \lim_{x \to 16} \frac{1}{x (\sqrt{x} + 4)} 
            = \boxed{ \frac{1}{128} } 
        \]

      \item[28]
        \[
          \lim_{h \to 0} \frac{(h+3)^{-1}-3^{-1}}{h} 
            = \lim_{h \to 0} -\frac{1}{3 h+9} 
            = \boxed{ - \frac{1}{9} } 
        \]

      \item[29]
        \begin{align*}
          \lim_{t \to 0} \frac{1}{t \sqrt{t+1}}-\frac{1}{t} 
            & = \lim_{t \to 0} \frac{1 - \sqrt{1 + t}}{t \sqrt{t+1}} \\
            & = \lim_{t \to 0} \frac{-1}{\sqrt{t+1} (1 + \sqrt{1 + t})} \\
            & = \boxed{ - \frac{1}{2} }
        \end{align*}

      \item[30]
        \begin{align*}
          \lim_{x \to 0} \frac{\sqrt{x^2+9}-5}{x+4} 
            &= \lim_{x \to 0} \frac{x^2+9-25}{\left(x+4\right) \left(\sqrt{x^2+9}+5 \right)} \\
            & = \lim_{x \to 0} \frac{x^2-16}{\left(x+4\right) \left(\sqrt{x^2+9}+5 \right)} \\
            & = \lim_{x \to 0} \frac{x-4}{\sqrt{x^2+9}+5} \\
            & = \boxed{ - \frac{4}{5} }
        \end{align*}

    \end{description}


  \else
    \vspace{11 cm}
    \begin{quote}
      \begin{em}
        TO DO
      \end{em}
    \end{quote}
    \hspace{1 cm} --Malcolm X
  \fi

\end{document}

