% no answer key
% \documentclass[letterpaper]{exam}

% answer key
\documentclass[letterpaper, landscape]{exam}
\usepackage{2in1, lscape} 
\printanswers

\usepackage{units} 
\usepackage{xfrac} 
\usepackage[fleqn]{amsmath}
\usepackage{float}
\usepackage{mdwlist}
\usepackage{booktabs}
\usepackage{cancel}
\usepackage{polynom}
\usepackage{caption}
\usepackage{fullpage}
\usepackage{comment}
\usepackage{enumerate}
\usepackage{graphicx}

\usepackage{mathtools} 

\newcommand{\dg}{\ensuremath{^\circ}} 
\newcommand{\sgn}{\operatorname{sgn}}

\everymath{\displaystyle}
\title{Calculus I \\ Homework Eleven \\ Section 3.3}
\author{}
\date{\today}

\begin{document}

  \maketitle

  \section{Homework}
    \begin{itemize*}
      \item read Section 3.3
      \item exercises: 1-15, 17-19, 23-24, 29, 31, 33, 35, 39-41, 49
    \end{itemize*}

  \ifprintanswers

  \section{Solutions}

  \begin{description}

    \item[1] 
      \[
        f'(x) = 6x + 2 \sin x
      \]

    \item[2] 
      \[
        f'(x) = \sqrt{x} \cos{x} + \frac{\sin{x}}{2 \sqrt{x}}
      \]

    \item[3] 
      \[
        f'(x) = \cos x - \frac{\csc^2 x}{2}
      \]

    \item[4] 
      \[
        y' = - 5 \sin x - 2 \cot x \csc x
      \]

    \item[5] 
      \[
        g'(t) = 3t^2 \cos t - t^3 \sin t
      \]

    \item[6] 
      \[
        g'(t) = \sec^2 t + 4 \sec t \tan t
      \]

    \item[7] 
      \[
        h'(\theta) = - \sin \theta + e^{\theta} \cot \theta - e^{\theta} \csc^2 \theta
      \]

    \item[8] 
      \[
        y' = e^x (c x + c - \sin x + \cos x)
      \]

    \item[9] 
      \[
        y' = \frac{ x \sec ^2 x - \tan x +  + 2}{( 2 - \tan x )^2}
      \]

    \item[10] 
      \[
        y' = \frac{x \cos x}{(x + \cos x)^2}
      \]

    \item[11] 
      \[
        f'(\theta) = \frac{\tan \theta \sec \theta}{(\sec \theta + 1)^2}
      \]

    \item[12] 
      \[
        y' = -\frac{1}{2} \sec ^2\left(\frac{\theta }{2}\right)
      \]

    \item[13] 
      \[
        y' = \frac{x \cos x - 2 \sin x}{x^3}
      \]

    \item[15] 
      \begin{align*}
        f(x)  & = x e^x \csc x \\
        f'(x) & = x \cdot \frac{d}{dx} \left( e^x \csc x \right) + e^x \csc x \\
              & = x \left( - e^x \csc x \cot x + e^x \csc x  \right)+ e^x \csc x \\
              & = e^x \csc x + e^x x \csc x - e^x x \csc x \cot x \\
      \end{align*}

    \item[17] 
      \begin{align*}
          \frac{d}{dx} (\csc x) & = \frac{d}{dx} \left( \frac{1}{\sin x} \right) \\
                                & = - \frac{\cos x}{\sin^2 x} \\
                                & = - \frac{\cos x}{\sin x} \cdot \frac{1}{\sin x} \\
                                & = - \cot x \csc x \\
      \end{align*}

    \item[18] 
      \begin{align*}
          \frac{d}{dx} (\sec x) & = \frac{d}{dx} \left( \frac{1}{\cos x} \right) \\
                                & = \frac{\sin x}{\cos^2 x} \\
                                & = \frac{\sin x}{\cos x} \cdot \frac{1}{\cos x} \\
                                & = \tan x \sec x \\
      \end{align*}

    \item[19] 
      \begin{align*}
          \frac{d}{dx} (\cot x) & = \frac{d}{dx} \left( \frac{\cos}{\sin x} \right) \\
                                & = \frac{- \sin^2 x - \cos^2 x}{\sin^2 x} \\
                                & = - \frac{\sin^2 x + \cos^2 x}{\sin^2 x} \\
                                & = - \frac{1}{\sin^2 x} \\
                                & = - \csc^2 x \\
      \end{align*}

    \item[23] 
      \begin{align*}
        y'    & = 1 - \sin x \\
        y'(0) & = 1 \\
        \\
        1     & = \frac{y - 1}{x - 0} \\
        y     & = x + 1 \\
      \end{align*}

    \item[24] 
      \begin{align*}
        y'    & = \frac{\sin x - \cos x}{(\sin x + \cos x)^2} \\
              & = \frac{\sin x - \cos x}{1 + 2 \sin x \cos x} \\
        y'(0) & = -1 \\
         \\
        -1 & = \frac{y - 1}{x - 0} \\
        y  & = x + 1 \\
      \end{align*}

    \item[29] 
      \begin{align*}
        H'(\theta)  & = \sin \theta + \theta \cos \theta \\
        H''(\theta) & = 2 \cos \theta - \theta \sin \theta \\
      \end{align*}

    \item[31] 
      approach one:
      \begin{align*}
        f(x)  & = \frac{\tan x - 1}{\sec x} \\
        f'(x) & = \frac{\sec^3 x - (\tan x - 1) \sec x \tan x}{\sec^2 x} \\
              & = \frac{\sec^2 x - (\tan x - 1) \tan x}{\sec x} \\
              & = \frac{\sec^2 x - \tan^2 x + \tan x}{\sec x} \\
              & = \frac{1 + \tan x}{\sec x} \\
              & = \cos x (1 + \tan x) \\
              & = \cos x + \sin x \\
      \end{align*}

      approach two:
      \begin{align*}
        f(x)  & = \frac{\tan x - 1}{\sec x} \\
              & = \cos x \left( \frac{\sin x}{\cos x} - 1 \right) \\
              & = \sin x - \cos x \\
        \\
        f'(x) & = \cos x + \sin x \\
      \end{align*}

    \item[33] 
      \begin{align*}
        f'(x)        & = 1 + 2 \cos x \\
        \\
        1 + 2 \cos x & = 0 \\
        \cos x       & = - \frac{1}{2} \\
        x            & = \left\{ \pm \frac{2 \pi}{3} \right\} \\
      \end{align*}

    \item[35] 
      \begin{enumerate}[(a)]
        \item 
          \begin{align*}
            x(t) & = 8 \sin t \\
            v(t) & = 8 \cos t \\
            a(t) & = - 8 \sin t \\
          \end{align*}

        \item 
          \begin{align*}
            x(2 \pi/3) & = \unit[4 \sqrt{3}]{cm} \\
            v(2 \pi/3) & = \unit[-2]{cm} \\
            a(2 \pi/3) & = \unit[- 4 \sqrt{3}]{cm} \\
          \end{align*}

          Since the velocity is negative, the block is moving to the left at 
          $t = \unit[2 \pi/3]{s}$.

      \end{enumerate}

    \item[39] 
      \begin{align*}
        \lim_{x \to 0} \frac{\sin 3x}{x} & = 3 \lim_{x \to 0} \frac{\sin 3x}{3x} \\
                                         & = \boxed{ 3 } \\
      \end{align*}

    \item[40] 
      \begin{align*}
        \lim_{x \to 0} \frac{\sin 4x}{\sin 6x} & = \frac{4}{6} \lim_{x \to 0} \frac{\sin 4x}{\sin 4x} \\
                                               & = \boxed{ \frac{2}{3} } \\
      \end{align*}

    \item[41] 
      \begin{align*}
        \lim_{x \to 0} \frac{\cos \theta - 1}{\sin \theta} 
          & = \lim_{x \to 0} \frac{\cos^2 \theta - 1}{\sin \theta (\cos \theta + 1)} \\
          & = \lim_{x \to 0} \frac{- \sin^2 \theta}{\sin \theta (\cos \theta + 1)} \\
          & = \lim_{x \to 0} \frac{- \sin \theta}{(\cos \theta + 1)} \\
          & = \boxed{ 0 } \\
      \end{align*}

    \item[49]
      \begin{enumerate}[(a)]
        \item 
          \begin{align*}
            \tan x                  & = \frac{\sin x}{\cos x} \\
            \frac{d}{dx} ( \tan x ) & = \frac{d}{dx} \left( \frac{\sin x}{\cos x} \right) \\
            \sec^2 x                & =  \frac{\cos^2 x + \sin^2 x}{\cos^2 x} \\
            \sec^2 x                & =  \frac{1}{\cos^2 x} \\
          \end{align*}

        \item
          \begin{align*}
            \sec x                  & = \frac{1}{\cos x} \\
            \frac{d}{dx} ( \sec x ) & = \frac{d}{dx} \left( \frac{1}{\cos x} \right) \\
            \sec x \tan x           & = \frac{\sin x}{\cos^2 x} \\
            % \sec x \tan x           & = \frac{\sin x}{\cos x} \cdot \frac{1}{\cos x} \\
            % \sec x \tan x           & = \tan x \cdot \sec x \\
          \end{align*}

        \item
          \begin{align*}
            \sin x + \cos x                  & = \frac{1 + \cot x }{\csc x} \\
            \frac{d}{dx} ( \sin x + \cos x ) & = \frac{d}{dx} \left( \frac{1 + \cot x }{\csc x}  \right) \\
            \cos x - \sin x                  & = \frac{ - \csc^3 x + (1 + \cot x) \cot x \csc x }{\csc^2 x} \\
                                             & = \frac{ - \csc^2 x + (1 + \cot x) \cot x }{\csc x} \\
                                             & = \frac{ \cot^2 x - \csc^2 x + \cot x }{\csc x} \\
            \cos x - \sin x                  & = \frac{ \cot x - 1 }{\csc x} \\
            % \cos x - \sin x                  & = ( \cot x - 1 ) \sin x \\
            % \cos x - \sin x                  & = ( \frac{\cos x}{\sin x} - 1 ) \sin x \\
            % \cos x - \sin x                  & = \cos x - \sin x \\
          \end{align*}
      \end{enumerate}

  \end{description}

  \else
    \vspace{10 cm}
    \begin{quote}
      \begin{em}
        The media, itself an arm of mega-corporate power, feeds the fear
        industry, so that people are primed like pumps to support wars on
        rumor, innuendo, legends and lies.
      \end{em}
    \end{quote}
    \hspace{2 cm} --Mumia Abu-Jamal
  \fi

\end{document}

