
\documentclass[fleqn,addpoints]{exam}

\usepackage{amsmath}
\usepackage{mdwlist}
\usepackage{graphicx}
\usepackage{cancel}
% \usepackage{polynom}
\usepackage{float}

\printanswers

\ifprintanswers
\usepackage{2in1, lscape}
\fi

\title{Math 113 Homework 20}
\author{}
\date{\today}

\begin{document}

\maketitle

\section{From the Book}

Read sections 10.1 and 10.2.

\begin{itemize*}
  \item pp. 497-498: 15-19, 30-34, 41, 45
  \item pp. pp 506-507: 6-10, 25-29, 43-44, 45, 49
\end{itemize*}

\ifprintanswers
\section{Pages 497-498}
\begin{description}

\item[15]
\begin{align*}
  x &= -3y \\
  7x-2y &= -69 \\
\end{align*}

substitute:
\begin{align*}
  7(-3y)-2y &= -69 \\
  -21y-2y &= -69 \\
  -23y &= -69 \\
  y &= 3 \\
\end{align*}

use $y$ to find $x$: $x = -3y = -3(3) = -9$.  

\vspace{0.2 cm}
\framebox{$(-9, 3)$}
\vspace{0.2 cm}

check:
\begin{align*}
  -9 &= -3(3) \\
  7(-9) - 2 (3) &= -69 \\
\end{align*}

\item[16]
\begin{align*}
  9x-2y &= -38 \\
  y &= -5x \\
\end{align*}

substitute:
\begin{align*}
  9x - 2(-5x) &= -38 \\
  19x &= -38 \\
  x &= -2 \\
\end{align*}

use $x$ to find $y$: $y = -5x = -5(-2) = 10$.  

\vspace{0.2 cm}
\framebox{$(-2, 10)$}
\vspace{0.2 cm}

check:
\begin{align*}
  9(-2)-2(10) &= -38 \\
  10 &= -5(-2) \\
\end{align*}

\item[17]
\begin{align*}
  2x+3y &= 11 \\
  3x-2y &= -3 \\
\end{align*}

solve one equation for $x$:
\begin{align*}
  2x+3y &= 11 \\
  2x &= 11 - 3y \\
  x &= \frac{11 - 3y}{2} \\
\end{align*}

substitute:
\begin{align*}
  3x-2y &= -3 \\
  3 \left( \frac{11 - 3y}{2} \right) -2y &= -3 \\
  3(11-3y) - 4y &= -6 \\
  33 - 13y &= -6 \\
  -13y &= -39 \\
  y &= 3 \\
\end{align*}

use $y$ to find $x$: $x = \dfrac{11 - 3y}{2} = \dfrac{11 - 3(3)}{2} = 1$.  

\vspace{0.2 cm}
\framebox{$(1, 3)$}
\vspace{0.2 cm}

check:
\begin{align*}
  2(1) + 3(3) &= 11 \\
  3(1) - 2(3) &= -3 \\
\end{align*}

\item[18]
\begin{align*}
  3x-4y &= -14 \\
  4x+3y &= 23 \\
\end{align*}

solve one equation for $x$:
\begin{align*}
  3x-4y &= -14 \\
  3x &= 4y-14 \\
  x &= \frac{4y-14}{3} \\
\end{align*}

substitute:
\begin{align*}
  4(\frac{4y-14}{3}) + 3y &= 23 \\
  4(4y-14) + 9y &= 69 \\
  25y &= 125 \\
   y &= 5 \\
\end{align*}

use $y$ to find $x$: $x = \dfrac{4(5) - 14}{3} = 2$

\vspace{0.2 cm}
\framebox{$(2, 5)$}
\vspace{0.2 cm}

check:
\begin{align*}
  3(2)-4(5) &= -14 \\
  4(2)+3(5) &= 23 \\
\end{align*}

\item[19]
\begin{align*}
  3x-4y &= 9 \\
  x &= 4y-1 \\
\end{align*}

substitute:
\begin{align*}
  3(4y-1)-4y &= 9 \\
  8y-3 &= 9 \\
  y &= \frac{3}{2} \\
\end{align*}

use $y$ to find $x$: $x = 4\left( \dfrac{3}{2} \right) - 1 = 5$

\vspace{0.2 cm}
\framebox{$(5, \dfrac{3}{2})$}
\vspace{0.2 cm}

check:
\begin{align*}
  3 \left( \dfrac{3}{2} \right)-4(5) &= 9 \\
  \dfrac{3}{2} &= 4(5)-1 \\
\end{align*}

\item[30]
\begin{align*}
  2x-y &= 9 \\
  7x+4y &= 1 \\
\end{align*}

solve one equation for $y$:
\begin{align*}
  2x-y &= 9 \\
  y &= 2x-9 \\
\end{align*}

substitute:
\begin{align*}
  7x+4(2x-9) &= 1 \\
  x &= \frac{37}{15}
\end{align*}

use $x$ to find $y$: $y = 2\left( \dfrac{37}{15} \right) - 9 = - \dfrac{61}{15}$

\vspace{0.2 cm}
\framebox{$(\dfrac{37}{15}, - \dfrac{61}{15})$}
\vspace{0.2 cm}

check:
\begin{align*}
  2\left( \frac{37}{15} \right) - \left( - \dfrac{61}{15} \right) &= 9 \\
  7\left( \frac{37}{15} \right) + 4\left( - \dfrac{61}{15} \right) &= 1 \\
\end{align*}

\item[31]
\begin{align*}
  3x+5y &= 22 \\
  4x - 7y &= -39 \\
\end{align*}

solve one equation for $x$:
\begin{align*}
  3x+5y &= 22 \\
  x &= \frac{22-5y}{3}
\end{align*}

substitute:
\begin{align*}
  4\left( \frac{22-5y}{3} \right) - 7y &= -39 \\
  y &= 5 \\
\end{align*}

use $y$ to find $x$: $x = \dfrac{22 - 5(5)}{3} = -1$

\vspace{0.2 cm}
\framebox{$(-1, 5)$}
\vspace{0.2 cm}

check:
\begin{align*}
  3(-1)+5(5) &= 22 \\
  4(-1) - 7(5) &= -39 \\
\end{align*}

\item[32]
\begin{align*}
  2x-3y &= -16 \\
  6x + 7y &= 16 \\
\end{align*}

solve one equation for $x$:
\begin{align*}
  2x-3y &= -16 \\
  x &= \frac{3}{2} y - 8 \\
\end{align*}

substitute:
\begin{align*}
  6 \left( \frac{3}{2}y - 8 \right) + 7y &= 16 \\
  9y - 48 + 7y &= 16 \\
  16y &= 54 \\
  y &= 4 \\
\end{align*}

use $y$ to find $x$: $x = \dfrac{3}{2}(4) - 8 = -2$

\vspace{0.2 cm}
\framebox{$(-2, 4)$}
\vspace{0.2 cm}

check:
\begin{align*}
  2(-2)-3(4) &= -16 \\
  6(-2) + 7(4) &= 16 \\
\end{align*}

\item[33]
\begin{align*}
  4x-5y &= 3 \\
  8x + 15y &= -24 \\
\end{align*}

solve one equation for $x$:
\begin{align*}
  4x-5y &= 3 \\
  x &= \frac{5y+3}{4} \\
\end{align*}

substitute:
\begin{align*}
  8x + 15y &= -24 \\
  8 \left( \frac{5y+3}{4} \right) + 15y &= -24 \\
  10y + 6 + 15y &= -24 \\
  y = - \frac{6}{5} \\
\end{align*}

use $y$ to find $x$: $x = \dfrac{5}{4} y + \dfrac{3}{4} 
  = \left( \dfrac{5}{4} \right) \left( - \dfrac{6}{5} \right) + \dfrac{3}{4} = - \dfrac{3}{4}$

\vspace{0.2 cm}
\framebox{$\left(- \dfrac{3}{4}, - \dfrac{6}{5}\right)$}
\vspace{0.2 cm}

check:
\begin{align*}
  4\left( -\frac{6}{5} \right)-5\left( - \frac{3}{4} \right) &= 3 \\
  8\left( -\frac{6}{5} \right) + 15\left( - \frac{3}{4} \right) &= -24 \\
\end{align*}

\item[34]
\begin{align*}
  2x+3y &= 3 \\
  4x-9y &= -4 \\
\end{align*}

solve one equation for $x$:
\begin{align*}
  2x+3y &= 3 \\
  x &= \frac{3 - 3y}{2}
\end{align*}

substitute:
\begin{align*}
  4 \left( \frac{3-3y}{2} \right) -9y &= -4 \\
  6 - 6y - 9y &= -4 \\
  y &= \frac{2}{3}
\end{align*}

use $y$ to find $x$: $x = \dfrac{3}{2} - \left( \dfrac{3}{2} \right)y 
  = \dfrac{3}{2} - \left( \dfrac{3}{2} \right) \left( \dfrac{2}{3} \right)
  = \dfrac{1}{2}$

\vspace{0.2 cm}
\framebox{$\left(\dfrac{1}{2}, \dfrac{2}{3} \right)$}
\vspace{0.2 cm}

check:
\begin{align*}
  2\left( \frac{1}{2} \right)+3\left( \frac{2}{3} \right) &= 3 \\
  4\left( \frac{1}{2} \right)-9\left( \frac{2}{3} \right) &= -4 \\
\end{align*}

\item[41]
\begin{align*}
  x+y &= 131 \\
  x &= 3y - 5 \\
\end{align*}

substitute:
\begin{align*}
  x+y &= 131 \\
  3y-5+y &= 131 \\
  y &= 34 \\
\end{align*}

use $y$ to find $x$: $x = 3y - 5 = 3(34) - 5 = 97$

\vspace{0.2 cm}
\framebox{$(97, 34)$}
\vspace{0.2 cm}

check:
\begin{align*}
  97 + 34 &= 31 \\
  3(34) - 5 &= 97 \\
\end{align*}

\item[45]
\begin{align*}
  L &= W + 7 \\
  2L + 2W &= 94 \\
\end{align*}

substitute:
\begin{align*}
  2L + 2W &= 94 \\
  L + W &= 47 \\
  W+7 + W &= 47 \\
  W &= 20 \\
\end{align*}

use $W$ to find $L$: $  L = W + 7 = 20 + 7 = 27$

check: $2(27) + 2(20) = 54 + 40 = 94$
\begin{align*}
\end{align*}


\end{description}

\section{Pages 506-507}
\begin{description}

\item[6]
\begin{align*}
  x-4y &= 29 \\
  3x+2y &= -11 \\    
  \\
  x-4y &= 29 \\
  6x+4y &= -22 \\
  \\
  7x &= 7 \\
  x &= 1 \\
\end{align*}

use $x$ to find $y$:
\begin{align*}
  x-4y &= 29 \\
  x - 4y &= 29 \\
  y &= -7 \\
\end{align*}

\vspace{0.2 cm}
\framebox{$(1, -7)$}
\vspace{0.2 cm}

check:
\begin{align*}
  1-4(-7) &= 29 \\
  3(1)+2(-7) &= -11 \\    
\end{align*}

\item[7]
\begin{align*}
  4x+7y &= -16 \\
  6x-y &= -24 \\
  \\
  4x+7y &= -16 \\
  42x-7y &= -168 \\
  \\
  46x &= -174 \\
  x &= -4
\end{align*}

use $x$ to find $y$:
\begin{align*}
  6(-4)-y &= -24 \\
  y &= 0 \\
\end{align*}

\vspace{0.2 cm}
\framebox{$(-4, 0)$}
\vspace{0.2 cm}

check:
\begin{align*}
  4(-4)+7(0) &= -16 \\
  6(-4)-0 &= -24 \\
\end{align*}

\item[8]
\begin{align*}
  6x+7y &= 17 \\
  3x+y &= -4 \\
  \\ 
  6x+7y &= 17 \\
  -6x - 2y &= 8 \\
  \\
  5y &= 25 \\
  y &= 5
\end{align*}

use $y$ to find $x$:
\begin{align*}
  3x+y &= -4 \\
  3x+5 &= -4 \\
  x &= -3 \\
\end{align*}

\vspace{0.2 cm}
\framebox{$(-3, 5)$}
\vspace{0.2 cm}

check:
\begin{align*}
  6(-3)+7(5) &= 17 \\
  3(-3)+(5) &= -4 \\
\end{align*}

\item[9]
\begin{align*}
  3x - 2y &= 5 \\
  2x+5y &= -3 \\
  \\
  -6x + 4y &= -10 \\
  6x + 15y &= -9 \\
  \\
  19y &= -19 \\
  y &= -1 \\
\end{align*}

use $y$ to find $x$:
\begin{align*}
  2x+5y &= -3 \\
  2x + 5(-1) &= -3 \\
  x &= 1 \\
\end{align*}

\vspace{0.2 cm}
\framebox{$(1, -1)$}
\vspace{0.2 cm}

check:
\begin{align*}
  3(1) - 2(-1) &= 5 \\
  2(1)+5(-1) &= -3 \\
\end{align*}

\item[10]
\begin{align*}
  4x+3y &= -4 \\
  3x-7y &= 34 \\
  \\
  12x + 9y &= -12 \\
  -12x + 28y &= -136 \\
  \\
  37y &= -148 \\
  y &= -4 \\
\end{align*}

use $y$ to find $x$:
\begin{align*}
  4x+3y &= -4 \\
  4x+3(-4) &= -4 \\
  x &= 2 \\
\end{align*}

\vspace{0.2 cm}
\framebox{$(2, -4)$}
\vspace{0.2 cm}

check:
\begin{align*}
  4(2)+3(-4) &= -4 \\
  3(2)-7(-4) &= 34 \\
\end{align*}

\item[25]
\begin{align*}
  5x-2y &= 1 \\
  10x - 4y &= 7 \\
  \\
  -10x + 4y &= -2 \\
  10x - 4y &= 7 \\
  \\
  0 &= 5
\end{align*}

There is no solution and these are {\em inconsistent} equations.

\item[26]
\begin{align*}
  4x+7y &= 2 \\
  9x - 2y &= 1 \\
  \\
  8x+14y &= 4 \\
  63x - 14y &= 7 \\
  \\
  71x &= 11 \\
  x &= \frac{11}{71}
\end{align*}

use $x$ to find $y$:
\begin{align*}
  4x+7y &= 2 \\
  4\left( \frac{11}{71} \right)+7y &= 2 \\
  y &= \frac{14}{71}
\end{align*}

\vspace{0.2 cm}
\framebox{$(\dfrac{11}{71}, \dfrac{14}{71})$}
\vspace{0.2 cm}

check:
\begin{align*}
  4\left( \frac{11}{71} \right)+7\left( \frac{14}{71} \right) &= 2 \\
  9\left( \frac{11}{71} \right) - 2\left( \frac{14}{71} \right) &= 1 \\
\end{align*}

\item[27]
\begin{align*}
  3x-2y &= 7 \\
  5x + 7y &= 1 \\
  \\
  15x-10y &= 35 \\
  -15x - 21y &= -3 \\
  \\
  -31y &= 32 \\
  y &= - \frac{32}{31} \\
\end{align*}

use $y$ to find $x$:
\begin{align*}
  3x-2y &= 7 \\
  3x-2\left( - \frac{32}{31} \right) &= 7 \\
  y &= \frac{51}{31} \\
\end{align*}

\vspace{0.2 cm}
\framebox{$\left( \dfrac{51}{31}, -\dfrac{32}{31} \right)$}
\vspace{0.2 cm}

check:
\begin{align*}
  3\left( - \frac{32}{31} \right)-2\left( \frac{51}{31} \right) &= 7 \\
  5\left( - \frac{32}{31} \right) + 7\left( \frac{51}{31} \right) &= 1 \\
\end{align*}

\item[28]
\begin{align*}
  2x-3y &= 4 \\
  y &= \frac{2}{3} x - \frac{4}{3}
\end{align*}

substitute:
\begin{align*}  
  2x-3y &= 4 \\
  2x - 3\left( \frac{2}{3} x - \frac{4}{3} \right) &= 4 \\
  2x - 2x + 4 &= 4 \\
  4 &= 4 \\
\end{align*}

These are {\em dependent} equations.

As another check, we can solve the first equation for $y$ and notice that we get the second equation:
\begin{align*}
  2x-3y &= 4 \\
  -3y &= -2x - 4 \\
  y &= \frac{2}{3} x + \frac{4}{3}
\end{align*}

\item[29]
\begin{align*}
  -2x + 5y &= -16 \\
  x &= \frac{3}{4} y + 1 \\
\end{align*}

substitute:
\begin{align*}
  -2x + 5y &= -16 \\
  -2\left( \frac{3}{4} y + 1 \right) + 5y &= -16 \\
  -3y - 4 + 10y &= -32 \\
  y &= -4 \\
\end{align*}

use $y$ to find $x$:
\begin{align*}
  x &= \frac{3}{4} y + 1 \\
  x &= \frac{3}{4} (-4) + 1 \\
  x &= -2 \\
\end{align*}

\vspace{0.2 cm}
\framebox{$(-2, -4)$}
\vspace{0.2 cm}

check:
\begin{align*}
  -2(-2) + 5(-4) &= -16 \\
  -2 &= \frac{3}{4} (-4) + 1 \\
\end{align*}

\item[43]
\begin{align*}
  \frac{3x+y}{2} + \frac{x-2y}{5} &= 8 \\
  \frac{x-y}{3} - \frac{x+y}{6} = \frac{10}{3} \\
  \\
  15x + 5y + 2x - 4y &= 80 \\
  2x - 2y - (x+y) &= 20 \\
  \\
  17x + y &= 80 \\
  x - 3y &= 20 \\
  \\
  51x + 3y &= 240 \\
  x - 3y &= 20 \\
  \\
  52x &= 260 \\
  x &= 5 \\
\end{align*}

use $x$ to find $y$:
\begin{align*}
  x - 3y &= 20 \\
  5 - 3y &= 20 \\
  -3y &= 15 \\
  y &= -5 \\
\end{align*}

\vspace{0.2 cm}
\framebox{$(5, -5)$}
\vspace{0.2 cm}

check:
\begin{align*}
  \frac{3(5)-5}{2} + \frac{5-2(-5)}{5} &= 8 \\
  \frac{5-(-5)}{3} - \frac{5-5}{6} = \frac{10}{3} \\
\end{align*}

\item[44]
\begin{align*}
  \frac{x-y}{4} - \frac{2x-y}{3} &= -\frac{1}{4} \\
  \frac{2x+y}{3} + \frac{x+y}{2} &= \frac{17}{6} \\
  \\
  3(x - y) - 4(2x-y) = 12 \left( - \frac{1}{4} \right) \\
  2(2x+y) + 3(x+y) &= 6 \left( \frac{17}{6} \right) \\
  \\
  3x - 3y - 8x + 4y = -3 \\
  4x + 2y + 3x + 3y &= 17 \\
  \\
  -5x + y &= -3 \\
  7x + 5y &= 17 \\
  \\ 
  25x - 5y &= 15 \\
   7x + 5y &= 17 \\
  \\
  32x &= 32 \\
  x &= 1 \\
\end{align*}

use $x$ to find $y$:
\begin{align*}
  -5x + y &= -3 \\
  -5(1) + y &= -3 \\
  y &= 2 \\
\end{align*}

\vspace{0.2 cm}
\framebox{$(1, 2)$}
\vspace{0.2 cm}

check:
\begin{align*}
  \frac{1-2}{4} - \frac{2(1)-2}{3} &= -\frac{1}{4} \\
  \frac{2(1)+2}{3} + \frac{1+2}{2} &= \frac{17}{6} \\
\end{align*}

\item[45]
If we let $x$ be the amount of 10\% solution and $y$ be the amount of 20\% solution, we have this system of equations:
\begin{align*}
  .1x + .2y &= .175 \cdot 20 \\
  x + y = 20 \\
  \\
  .1x + .2y &= 3.5 \\
  x + y = 20 \\
  \\
  x + 2y &= 35 \\
  -x - y &= -20 \\
  \\
  y &= 15
\end{align*}

use $y$ to find $x$:
\begin{align*}
  x + y &= 20 \\
  x + 15 &= 20 \\
  x &= 5 \\
\end{align*}

check: $.1(5) + .2(15) = .175 \cdot 20$
\begin{align*}
\end{align*}

\item[49]
If we let $x$ be the number of double rooms and $y$ be the number of single rooms, we have this system of equations:
\begin{align*}
  42x + 22y &= 2,010 \\
  x + y &= 55 \\
\end{align*}

If we solve the second equation for $y$, we can use substitution:
\begin{align*}
  42x + 22(55-x) &= 2,010 \\
  21x + 11(55-x) &= 1,050 \\
  21x + 605 - 11x &= 1,050 \\
  10x &= 400 \\
  x &= 15
\end{align*}

use $x$ to find $y$: $y = 55-x = 55-15 = 40$

check: $42(15) + 22(40) = 2,010$

\end{description}
\fi


\section{Review Problems}

\begin{questions}
\question 
Evaluate: $16^{\frac{3}{2}}$

\begin{solution}
  $16^{\frac{3}{2}} = (\sqrt{16})^3 = 4^3 = 64$
\end{solution}

\question 
Evaluate: $27^{-\frac{2}{3}}$

\begin{solution}

\begin{align*}
  27^{-\frac{2}{3}} &= (3^3)^{-\frac{2}{3}} \\
  &= 3^{-2} \\
  &= \frac{1}{9} \\
\end{align*}
\end{solution}

\question 
Evaluate: $\sqrt{5} \sqrt{20}$
\begin{solution}
  $\sqrt{5} \sqrt{20} = \sqrt{5 \cdot 20} = \sqrt{100} = 10$
\end{solution}

\question 
Simplify: $\left( \dfrac{x^{\frac{1}{2}}}{x^{\frac{1}{3}}} \right)^2$

\begin{solution}
\[
  \left( \frac{x^{\frac{1}{2}}}{x^{\frac{1}{3}}} \right)^2
  = \frac{x}{x^{\frac{2}{3}}}
  = \frac{x^{\frac{3}{3}}}{x^{\frac{2}{3}}}
  = x^{\frac{1}{3}}
\]
\end{solution}

\question 
Simplify: $\sqrt[4]{16x^5y^8}$
\begin{solution}
\[
  \sqrt[4]{16x^5y^8} = \sqrt[4]{2^4x^4xy^8} = 2xy^2\sqrt[4]{x}
\]

\end{solution}

\question
Rationalize the denominator: $\dfrac{3}{\sqrt[3]{9y}}$
\begin{solution}
\[
  \frac{3}{\sqrt[3]{9y}} = \frac{3}{\sqrt[3]{3^2y}} \left( \frac{\sqrt[3]{3y^2}}{\sqrt[3]{3y^2}} \right)
  = \frac{\cancel{3} \sqrt[3]{3y^2}}{\cancel{3}y}
  = \frac{\sqrt[3]{3y^2}}{y}
\]
\end{solution}

\question
Rationalize the denominator: $\dfrac{10}{\sqrt{6} - \sqrt{2}}$

\begin{solution}

\begin{align*}
  \frac{10}{\sqrt{6} - \sqrt{2}} \left( \frac{\sqrt{6} + \sqrt{2}}{\sqrt{6} + \sqrt{2}} \right)
  &= \frac{10 \sqrt{6} + 10 \sqrt{2}}{6-4} \\
  &= \frac{10\sqrt{6} + 10\sqrt{2})}{2} \\
  &= 5\sqrt{6} + 5\sqrt{2} \\
\end{align*}
\end{solution}

\question
Subtract: $5 \sqrt{3x} - 3 \sqrt{75x}$

\begin{solution}
\begin{align*}
  5 \sqrt{3x} - 3 \sqrt{75x} &= 5 \sqrt{3x} - 3 \sqrt{5^2 \cdot 3x} \\
  &= 5 \sqrt{3x} - 15 \sqrt{3x} \\
  &= -10\sqrt{3x} \\
\end{align*}

\end{solution}

\question
Multiply and simlplify: $\sqrt{5}(x \sqrt{15} + 3)$

\begin{solution}
\begin{align*}
  \sqrt{5}(x \sqrt{15} + 3) &= x \sqrt{5 \cdot 5 \cdot 3} + 3\sqrt{5} \\
  &= 5x\sqrt{3} + 3\sqrt{5} 
\end{align*}
\end{solution}

\question
Solve: $\sqrt{3y} - 6 = 3$

\begin{solution}
\begin{align*}
  \sqrt{3y} - 6 &= 3 \\
  \sqrt{3y} &= 9 \\
  3y &= 81 \\
  y &= 27 \\
\end{align*}

check: $\sqrt{3 \cdot 27} - 6 = \sqrt{81} - 6 = 9 - 6 = 3$
\end{solution}

\question
Solve: $\sqrt{x^2-1}  = x - 2$

\begin{solution}
\begin{align*}
  \sqrt{x^2-1} &= x - 2 \\
  x^2-1 &= (x - 2)^2 \\
  x^2-1 &= x^2 - 4x + 4 \\
  -1 &= -4x + 4 \\
  0 &= -4x + 5 \\
  4x &=  5 \\
  x &=  \frac{5}{4} \\
\end{align*}

check:
\begin{align*}
  \sqrt{x^2-1} &= x - 2 \\
  \sqrt{\left( \frac{5}{4} \right)^2-1} &? \frac{5}{4} - 2 \\
  \sqrt{\frac{9}{16}} &? \frac{5}{4} - \frac{8}{4} \\
  \frac{3}{4} &\neq -\frac{3}{4} \\
\end{align*}

So there is no solution.

\end{solution}

\question
Solve: $\sqrt{x} - x + 6 = 0$

\begin{solution}
\begin{align*}
  \sqrt{x} - x + 6 &= 0 \\
  \sqrt{x} &= x - 6 \\
  x &= (x - 6)^2 \\
  x &= x^2 - 12x + 36 \\
  x^2 - 13x + 36 &= 0 \\
  (x-9)(x-4) &= 0 \\
\end{align*}

$x = \{ 4, 9 \}$

check:
\begin{align*}
  \sqrt{9} - 9 + 6 &= 0 \\
  \sqrt{4} - 4 + 6 \neq 0 \\
\end{align*}

Only $9$ works, so this is the only solution.

\end{solution}

\question
Simplify: $(3-2i)(1+5i)$

\begin{solution}
\begin{align*}
  (3-2i)(1+5i) &= 3 - 3i + 15i - 10i^2 \\
  &= 3 + 12i + 10 \\
  &= 13 + 12i \\
\end{align*}
\end{solution}

\question
Write in standard form: $\dfrac{5-2i}{3+i}$

\begin{solution}
\begin{align*}
  \frac{5-2i}{3+i} \left( \frac{3-i}{3-i} \right) &= \frac{15 - 6i - 5i + 2i^2}{9 - i^2} \\
  &= \frac{15 - 11i - i}{9+1} \\
  &= \frac{13 - 11i}{10} \\
  &= \frac{13}{10} - \frac{11}{10}i
\end{align*}

\end{solution}

\end{questions}

\ifprintanswers
\else
\vspace{0.5 in}

\begin{em}
Great people never lose their child's heart.
\end{em}

\vspace{0.1 in}
\hspace{0.5 in} -- Mencius 

\fi

\end{document}

