% no answer key
% \documentclass[letterpaper]{exam}

% answer key
\documentclass[letterpaper, landscape]{exam}
\usepackage{2in1, lscape} 
\printanswers

\usepackage{units} 
\usepackage{xfrac} 
\usepackage[fleqn]{amsmath}
\usepackage{float}
\usepackage{mdwlist}
\usepackage{booktabs}
\usepackage{cancel}
\usepackage{polynom}
\usepackage{caption}
\usepackage{fullpage}
\usepackage{comment}
\usepackage{enumerate}
\usepackage{graphicx}

\usepackage{mathtools} 

\newcommand{\dg}{\ensuremath{^\circ}} 
\newcommand{\sgn}{\operatorname{sgn}}

\everymath{\displaystyle}
\title{Calculus I \\ Homework Thirteen \\ Section 3.5}
\author{}
\date{\today}

\begin{document}

  \maketitle

  \section{Homework}
    \begin{itemize*}
      \item read Section 3.5
      \item exercises: 5-15, 21-25, 33-35, 45-47, 53
    \end{itemize*}

  \ifprintanswers

  \section{Solutions}

  \begin{description}

    \item[5] 
      \[
        y' = - \frac{x^2}{y^2} 
      \]


    \item[6] 
      \[
        y' = -2 \frac{\sqrt{y}}{\sqrt{x}} 
      \]

    \item[7] 
      \[
        y' = \frac{2x - y}{2y - x}
      \]

    \item[8] 
      \[
        y' = \frac{ - 6x^2 - 2xy + y^3}{x \left(x - 3y^2 \right)} 
      \]

    \item[9] 
      \[
        y' = \frac{-5 x^4-4 x^3 y+3 y^2}{x^4-6 x y+3 y^2}
      \]

    \item[10] 
      \[
        y' = \frac{y \left(2x y^2 - e^x\right)}{ - 3x^2 y^2 + e^x - 5 y^4}
      \]

    \item[11] 
      \[
        y' = \frac{ - 2x y^2 - \sin (y)}{x (2x y + \cos (y))}
      \]

    \item[12] 
      \[
        y' = \frac{\sec \left( x y^2 \right) - y^2 }{2x y}
      \]

    \item[13] 
      \[
        y' = \tan x \tan y
      \]

    \item[14] 
      \[
        y' = \frac{2x y \cos x^2 - \sin y^2}{2x y \cos y^2 - \sin x^2}
      \]

    \item[15] 
      \[
        y' = \frac{y \left( e^{x/y} - y \right)}{x e^{x/y} - y^2}
      \]

    \item[21] 
      \begin{align*}
        y'(x) & = - \frac{2x [f(x)]^3}{3x^2 [f(x)]^2 + 1} \\
        y'(1) & = \boxed{ - \frac{16}{13} } \\
      \end{align*}

    \item[22] 
      find $g'(x)$ by implicit differentiation:
      \[
        g'(x) = \frac{2x - \sin (g(x)) }{x \cos (g(x)) + 1}
      \]

      find $g(0)$:
      \begin{align*}
        g(0) + 0 \sin(g(0)) & = 0 \\
        g(0)                & = 0 \\
      \end{align*}

      find $g'(0)$:
      \begin{align*}
        g'(0) & = \frac{2 \cdot 0 - \sin (0) }{0 \cdot \cos (0) + 1} \\
              & = \boxed{ 0 } \\
      \end{align*}

    \item[23] 
      \[
        \frac{dx}{dy} = \frac{-2 x^4 y+x^3-6 x y^2}{y \left(4 x^3 y-3 x^2+2 y^2\right)}
      \]

    \item[25] 
      \begin{align*}
        y'       & = \frac{ - 2x - y}{x + 2 y} \\
        y'(1, 1) & = -1 \\
        \\
        -1       & = \frac{y - 1}{x - 1} \\
        y        & = 2 - x \\
      \end{align*}

    \item[33]
      \begin{align*}
        y'  & = - \frac{9x}{y} \\
        y'' & = \frac{9xy' - 9y}{y^2} \\
      \end{align*}

    \item[34] 
      \begin{align*}
        y'  & = - \frac{\sqrt{y}}{\sqrt{x}} \\
        y'' & = \frac{x^{3/2} y'^2 + y^{3/2}}{2x^{3/2} y}
      \end{align*}

    \item[35] 
      \begin{align*}
        \frac{x^2}{a^2} + \frac{y^2}{b^2} & = 1 \\
        \frac{2x}{a^2} + \frac{2yy'}{b^2} & = 0 \\
        % \frac{2yy'}{b^2}                  & = -\frac{2x}{a^2} \\
        y'                                & = - \frac{xb^2}{ya^2} \\
      \end{align*}


      find the equation of the line:
      \begin{align*}
        - \frac{x_0 b^2}{y_0 a^2} &= \frac{y - y_0}{x - x_0} \\
      \end{align*}

    \item[45] 
      \[
        f'(x) = \frac{1}{2 \sqrt{x} (x + 1)}
      \]

    \item[46] 
      \[
        f'(x) = \frac{1}{2 \left(x^2 + 1\right) \sqrt{\frac{x}{\tan }}}
      \]

    \item[47] 
      \[
        f'(x) = \frac{2}{\sqrt{1-(2 x+1)^2}}
      \]

    \item[53] 
      \[
        f'(x) = - \frac{2 e^{2x}}{\sqrt{1 - e^{4x}}}
      \]

  \end{description}

  \else
    \vspace{10 cm}
    \begin{quote}
      \begin{em}
        TO DO
      \end{em}
    \end{quote}
    \hspace{2 cm} --TO DO
  \fi

\end{document}

