
\documentclass[fleqn,addpoints]{exam}

\usepackage{amsmath}
\usepackage{graphics}
\usepackage{cancel}
\usepackage{polynom}
\usepackage{mdwlist}

\printanswers

\ifprintanswers
\usepackage{2in1, lscape}
\fi

\title{Math 113 Homework 14}
\author{}
\date{\today}

\begin{document}

\maketitle

\ifprintanswers
\else
\section{Chapter Five Test}

The {\em Chapter 5} test will be next week.  See the {\em Study Guide} for a summary of material from this chapter.

\fi

\section{From the Book}

\begin{itemize*}
  \item pp. 267-269: 15-24, 31-35, 50-54, 60-64, 75-79, 85-89
  \item pp. 273-274: 7-16, 25-29, 33-42, 51, 55, 56
\end{itemize*}

\ifprintanswers
\section{Pages 267-269}
\begin{itemize}

\item[15]
\[
  27^{\frac{4}{3}} = (\sqrt[3]{27})^4 = 3^4 = 81
\]

\item[16]
\[
  4^{\frac{7}{2}} = (\sqrt{4})^7 = 2^7 = 128
\]

\item[17]
\[
  (-1)^{\frac{7}{3}} = (\sqrt[3]{-1})^7= -1
\]

\item[18]
\[
  (-8)^{\frac{4}{3}} = (\sqrt[3]{-8})^4 = (-2)^4 = 16
\]

\item[19]
\[
  -4^{\frac{5}{2}} = -(\sqrt{4})^5 = -2^5 = -32
\]

\item[20]
\[
  -16^{\frac{3}{2}} = -(\sqrt{16})^3 = -4^3 = -64
\]

\item[21]
\[
  \left( \frac{27}{8} \right)^{\frac{4}{3}} = \left( \sqrt[3]{\frac{27}{8}} \right)^4 = \left( \frac{3}{2} \right)^4 = \frac{81}{16}
\]

\item[22]
\[
  \left( \frac{8}{125} \right)^{\frac{2}{3}} = \left( \sqrt[3]{\frac{8}{125}} \right)^2 = \left( \frac{2}{5} \right)^2 = \frac{4}{25}
\]

\item[23]
\[
  \left( \frac{1}{8} \right)^{-\frac{2}{3}} = \frac{1}{8^{-\frac{2}{3}} } = 8^{\frac{2}{3}} = (\sqrt[3]{8})^2 = 4
\]

\item[24]
\[
  \left( - \frac{1}{27} \right)^{-\frac{2}{3}} = \frac{1}{(-27)^{-\frac{2}{3}} } = (-27)^{\frac{2}{3}} = (\sqrt[3]{-27})^2 = 9
\]

\item[31]
\[
  x^{\frac{4}{3}} = \sqrt[3]{x^4}
\]

\item[32]
\[
  x^{\frac{2}{5}} = \sqrt[5]{x^2}
\]

\item[33]
\[
  3x^{\frac{1}{2}} = 3 \sqrt{x}
\]

\item[34]
\[
  5x^{\frac{1}{4}} = 5 \sqrt[4]{x}
\]

\item[35]
\[
  (2y)^\frac{1}{3} = \sqrt[3]{2y}
\]

\item[50]
\[
  \sqrt[5]{x^2y^4} = x^{\frac{2}{5}} y^{\frac{4}{5}}
\]

\item[51]
\[
  \sqrt[4]{a^2b^3} = a^{\frac{2}{4}} b^{\frac{3}{4}} = a^{\frac{1}{2}} b^{\frac{3}{4}}
\]

\item[52]
\[
  \sqrt[6]{ab^5} = a^{\frac{1}{6}} b^{\frac{5}{6}}
\]

\item[53]
\[
  \sqrt[5]{(2x-y)^3} = (2x-y)^{\frac{3}{5}}
\]

\item[54]
\[
  \sqrt[7]{(3x-y)^4} = (3x-y)^{\frac{4}{7}}
\]

\item[60]
\[
  (3x^{\frac{1}{4}})(5x^{\frac{1}{3}}) = 15x^{\frac{1}{4} + \frac{1}{3}} = 15x^{\frac{3}{12} + \frac{4}{12}} = 15x^{\frac{7}{12}}
\]

\item[61]
\[
  (y^{\frac{2}{3}})(y^{-\frac{1}{4}}) = y^{\frac{2}{3} - \frac{1}{4}} = y^{\frac{8}{12} - \frac{3}{12}} = y^{\frac{5}{12}}
\]

\item[62]
\[
  (y^{\frac{3}{4}})(y^{- \frac{1}{2}}) = y^{\frac{3}{4} - \frac{1}{2}} = y^{\frac{1}{4}}
\]

\item[63]
\[
  (x^{\frac{2}{5}}) (4x^{-\frac{1}{2}}) = 4x^{\frac{2}{5} - \frac{1}{2}} = 4x^{\frac{4}{10} - \frac{5}{10}} 
  = 4x^{-\frac{1}{10}} = \frac{4}{x^{\frac{1}{10}}}
\]

\item[64]
\[
  (2x^{\frac{1}{3}})(x^{-\frac{1}{2}}) 
  = 2x^{\frac{1}{3} - \frac{1}{2}} 
  = 2x^{\frac{2}{6} - \frac{3}{6}} 
  = 2x^{-\frac{1}{6}} 
  = \frac{2}{x^{\frac{1}{6}}}
\]

\item[75]
\[
  \left( \frac{x^2}{y^3} \right)^{- \frac{1}{2}}
  = \frac{x^{-1}}{y^{-\frac{3}{2}}} 
  = \frac{y^{\frac{3}{2}}}{x}
\]

\item[76]
\[
  \left( \frac{a^3}{b^{-2}} \right)^{- \frac{1}{3}}
  = \frac{a^{-1}}{b^{\frac{2}{3}}} 
  = \frac{1}{ab^{\frac{2}{3}}} 
\]

\item[77]
\[
  \left( \frac{18x^{\frac{1}{3}}}{9x^{\frac{1}{4}}} \right)^2
  = \left( \frac{2x^{\frac{1}{3}}}{x^{\frac{1}{4}}} \right)^2
  = (2x^{\frac{1}{3} - \frac{1}{4}})^2
  = (2x^{\frac{4}{12} - \frac{3}{12}})^2
  = (2x^{\frac{1}{12}})^2
  = 4 x^{\frac{1}{6}}
\]

\item[78]
\[
  \left( \frac{72x^{\frac{3}{4}}}{6x^{\frac{1}{2}}} \right)^2
  = ( 12x^{\frac{3}{4} - \frac{1}{2}} )^2
  = ( 12x^{\frac{1}{4}} )^2
  = 144x^{\frac{1}{2}}
\]

\item[79]
\[
  \left( \frac{60a^{\frac{1}{5}}}{15a^{\frac{3}{4}}} \right)^2
  = ( 4a^{\frac{1}{5} - \frac{3}{4}} )^2
  = ( 4a^{\frac{4}{20} - \frac{15}{20}} )^2
  = ( 4a^{- \frac{11}{20}} )^2
  = 16a^{- \frac{11}{10}}
  = \frac{16}{a^{\frac{11}{10}}}
\]

\item[85]
\[
  \frac{\sqrt[3]{3}}{\sqrt[4]{3}}
  = \frac{3^{\frac{1}{3}}}{3^{\frac{1}{4}}}
  = 3^{\frac{1}{3} - \frac{1}{4}}
  = 3^{\frac{4}{12} - \frac{3}{12}}
  = 3^{\frac{1}{12}}
  = \sqrt[12]{3}
\]

\item[86]
\[
  \frac{\sqrt{2}}{\sqrt[3]{2}}
  = \frac{2^{\frac{1}{2}}}{2^{\frac{1}{3}}}
  = 2^{\frac{1}{2} - \frac{1}{3}}
  = 2^{\frac{1}{6}}
  = \sqrt[6]{2}
\]

\item[87]
\[
  \frac{\sqrt[3]{8}}{\sqrt[4]{4}}
  = \frac{2}{\sqrt[4]{4}}
  = \frac{2}{\sqrt[2^2]{4}}
  = \frac{2}{\sqrt[4]{2^2}}
  = \frac{2}{2^{\frac{2}{4}}}
  = \frac{2}{2^{\frac{1}{2}}}
  = 2^{1 - \frac{1}{2}}
  = 2^{\frac{1}{2}}
  = \sqrt{2}
\]

\item[88]
\[
  \frac{\sqrt{9}}{\sqrt[3]{3}}
  = \frac{3}{3^{\frac{1}{3}}}
  = 3^{1 - \frac{1}{3}}
  = 3^{\frac{2}{3}}
\]

\item[89]
\[
  \frac{\sqrt[4]{27}}{\sqrt{3}}
  = \frac{\sqrt[4]{3^3}}{\sqrt{3}}
  = \frac{3^{\frac{3}{4}}}{3^{\frac{1}{2}}}
  = 3^{\frac{3}{4} - \frac{1}{2}}
  = 3^{\frac{1}{4}}
\]

\section{Pages 273-274}

\item[7]
\[
  40,000,000 = (4)(10^7)
\]

\item[8]
\[
  500,000,000 = (5)(10^8)
\]

\item[9]
\[
  376.4 = (3.764)(10^2)
\]

\item[10]
\[
  9,126.21 = (9.12621)(10^3)
\]

\item[11]
\[
  0.347 = (3.47)(10^{-1})
\]

\item[12]
\[
  0.2165 = (2.165)(10^{-1})
\]

\item[13]
\[
  0.0214 = (2.14)(10^{-2})
\]

\item[14]
\[
  0.0037 = (3.7)(10^{-3})
\]

\item[15]
\[
  0.00005 = (5)(10^{-5})
\]

\item[16]
\[
  0.00000082 = (8.2)(10^{-7})
\]

\item[25]
\[
  (3.14)(10^{10}) = 31,400,000,000
\]

\item[26]
\[
  (2.04)(10^{12}) = 2,040,000,000,000
\]

\item[27]
\[
  (4.3)(10^{-1}) = 0.43
\]

\item[28]
\[
  (5.2)(10^{-2}) = 0.052
\]

\item[29]
\[
  (9.14)(10^{-4}) = 0.000914
\]

\item[33]
\[
  (0.0037)(0.00002) = (3.7)(10^{-3})((2)(10^{-5})) = (7.4)(10^{-8}) = 0.000000074
\]

\item[34]
\[
  (0.00003)(0.00025) = (3)(10^{-5})(2.5)(10^{-4}) = (7.5)(10^{-9}) = 0.0000000075
\]

\item[35]
\[
  (0.00007)(11,000) = (7)(10^{-5})(1.1)(10^{4}) = (7.7)(10^{-1}) = 0.77
\]

\item[36]
\[
  (0.000004)(120,000) = (4)(10^{-6})(1.2)(10^{5}) = (4.8)(10^{-1}) = 0.48
\]

\item[37]
\[
  \frac{360,000,000}{0.0012} = \frac{(3.6)(10^8)}{(1.2)(10^{-3})} = (3)(10^{11}) = 300,000,000,000
\]

\item[38]
\[
  \frac{66,000,000,000}{0.022} = \frac{(6.6)(10^{10})}{(2.2)(10^{-2})} = (3)(10^{12}) = 3,000,000,000,000
\]

\item[39]
\[
  \frac{0.000064}{16,000} = \frac{(6.4)(10^{-5})}{(1.6)(10^{4})} = (4)(10^{-9}) = 0.000000004
\]

\item[40]
\[
  \frac{0.00072}{0.0000024} = \frac{(7.2)(10^{-4})}{(2.4)(10^{-6})} = (3)(10^{2}) = 300
\]

\item[41]
\[
  \frac{(60,000)(0.006)}{(0.0009)(400)} = \frac{(6)(10^{4})(6)(10^{-3})}{(9)(10^{-4})(4)(10^{2})}
  = \frac{(36)(10^{1})}{(36)(10^{-2})}
  = 10^3 = 1,000
\]

\item[42]
\[
  \frac{(0.00063)(960,000)}{(3,200)(0.0000021)}
  = \frac{(6.3)(10^{-4}) (9.6)(10^{5})}{(3.2)(10^{3})(2.1)(10^{-6})}
  = 3 \cdot 3 (10^4) = (9)(10^4) = 90,000
\]

% \item[43]
% \[
%   \frac{(0.0045)(60,000)}{(1,800)(0.00015)}
%   = \frac{(4.5)(10^{-3})(6)(10^{4})}{(1.8)(10^{3})(1.5)(10^{-4})}
%   = (10)(10^{2}) = 1,000
% \]

\item[51]
\[
  602,000,000,000,000,000,000,000 = (6.02)(10^{23})
\]

\item[55]

The numbers are: $5,700,000,000,000 = (5.7)(10^{12})$ and $275,000,000 = (2.75)(10^{8})$.

The average is
\[
  \frac{(5.7)(10^{12})}{(2.75)(10^{8})} = (2.07)(10^{4}) = 20,700
\]

So each person owed approximately \$20,700.  I imagine the total is higher now.

\item[56]
\[
  \frac{140,000,000}{410,000} = \frac{(1.4)(10^8)}{(4.1)(10^5)} \approx (3.41)(10^3) = 341
\]

% \item[57]
% \[
%   \frac{1}{12} \cdot (1.66)(10^{-27}) = (0.138)(10^{-27}) = (1.38)(10^{-28})
% \]
\end{itemize}

\fi

\ifprintanswers
\else
\section{Review}

To review for the test, you should take a look at the {\em Study Guide} and the {\em Chapter 5} {\em Review Problems} and 
{\em Sample Test}.

\fi

% \section{Extra Credit}

% Review for the {\em Chapter 5 test
% \begin{questions}
% \question
% question here

% \end{questions}

\ifprintanswers
\else
\vspace{4 in}

{\em Confusion is not a bad thing.  It is the first step towards understanding.}

\hspace{0.5 in} --Edward Teller

\fi

\end{document}

