% no answer key
% \documentclass[letterpaper]{exam}

% answer key
\documentclass[letterpaper, landscape]{exam}
\usepackage{2in1, lscape} 
\printanswers

\usepackage{units} 
\usepackage{xfrac} 
\usepackage[fleqn]{amsmath}
\usepackage{float}
\usepackage{mdwlist}
\usepackage{booktabs}
\usepackage{cancel}
\usepackage{polynom}
\usepackage{caption}
\usepackage{fullpage}
\usepackage{comment}
\usepackage{enumerate}
\usepackage{graphicx}

\usepackage{mathtools} 

\newcommand{\dg}{\ensuremath{^\circ}} 
\newcommand{\sgn}{\operatorname{sgn}}

\everymath{\displaystyle}
\title{Calculus I \\ Homework Ten \\ Section 3.2}
\author{}
\date{\today}

\begin{document}

  \maketitle

  \section{Homework}
    \begin{itemize*}
      \item read Section 3.2
      \item exercises: 3-10, 13-14, 17-18, 21-22, 25-27, 29, 31-33, 41,43, 45, 49, 58
    \end{itemize*}

  \ifprintanswers

  \section{Solutions}

  \begin{description}

    \item[3] 
      \begin{align*}
        f'(x) & = \left( x^3 + 2x \right) e^x + \left( 3x^2 + 2 \right) e^x \\
              & = \boxed{ e^x \left( x^3 + 3x^2 + 2x + 2 \right) } \\
      \end{align*}

    \item[4] 
      \begin{align*}
        f'(x) & = x^{1/2} e^x + \frac{1}{2} x^{-1/2} e^x \\
        & = \boxed{ e^x \left( x^{1/2} + \frac{1}{2} x^{-1/2} \right) } \\
      \end{align*}

    \item[5] 
      \begin{align*}
        f(x)  & = e^x x^{-2} \\
        f'(x) & = e^x x^{-2} + e^x \left( -2 x^{-3} \right) \\
              & = \boxed{ e^x \left( x^{-2} -2 x^{-3} \right) } \\
      \end{align*}

    \item[6] 
      \[
        f'(x) = \boxed{ \frac{e^x x}{(x + 1)^2} }      
      \]

    \item[7] 
      \[
        f'(x) = \boxed{ \frac{5}{(2x + 1)^2} }
      \]

    \item[8] 
      \[
        f'(t) = \boxed{ \frac{ - 2t^2 + 8  }{\left( t^2 + 4 \right)^2} }
      \]
      
    \item[9] 
      \[
        V'(x) = \boxed{ 14x^6 - 4x^3 - 6 } 
      \]
      
    \item[10] 
      \[
        Y'(u) = \boxed{ 3u^2 + 2u + 2u^{-2} } 
      \]
      
    % \item[11] 
    %   \[
    %     F'(y) = 9y^{-4} + 14y^{-2} + 5
    %   \]
      
    % \item[12] 
    %   \[
    %     R'(t) = \frac{-1}{2 \sqrt{t}} 
    %       \left( e^t + t \right) + \left( e^t + 1 \right) (\sqrt{t} - 3)
    %   \]

    \item[13] 
      \[
        y' = \boxed{ \frac{ -x^4 + 3x^2 }{\left( x^2 - 1 \right)^2} }
      \]
      
    \item[14] 
      \[
        y' = \boxed{ \frac{-2x^3 - 3x^2 - 3}{\left( x^3 + x - 2 \right)^2} }
      \]
      
    % \item[15] 
    %   \[
    %     y' = \frac{ -2t^5 + 14t }{\left( \left( t^4 - 3t^2 + 1 \right)^2 \right)^2}
    %   \]
      
    % \item[16] 
    %   \[
    %     y' =  - \frac{t + 1}{(t - 1)^3}
    %   \]

    \item[17] 
      \[
        y' = \boxed{ e^r \left( r^2 - 2 \right) }
      \]

    \item[18] 
      \[
        y' = \boxed{ \frac{-1 - k e^s}{\left( s + k e^s \right)^2} }
      \]

    \item[21] 
      \[
        y' = \boxed{ \frac{t^{1/2} + 4}{\left( t^{1/2} + 2 \right)^2} }
      \]

    \item[22] 
      \begin{align*}
        g(t)  & = \frac{t - t^{1/2}}{t^{1/3}} \\
              & = t^{2/3} - t^{1/6} \\
        \\
        g'(t) & = \boxed{ \frac{2}{3} t^{-1/3} - \frac{1}{6} t^{-5/6} } \\
      \end{align*}
      % \[
      %   y' = \boxed{ \frac{4 t^{1/2} - 1}{6t^{5/6}} }
      % \]

    \item[25] 
      \begin{align*}
        f(x)  & = \frac{x}{x + \cfrac{c}{x} } \\
              & = \frac{x^2}{x^2 + c} \\
        \\
        f'(x) & = \boxed{ \frac{2 c x}{\left( x^2 + c \right)^2} }
      \end{align*}

    \item[26] 
      \[
        y' = \boxed{ \frac{a d - b c}{(c x + d)^2} }
      \]

    \item[27]
      \begin{align*}
        f(x)   & = x^4 e^x \\
        f'(x)  & = x^4 e^x + 4x^3 e^x \\
               & = \boxed{ e^x \left( x^4 + 4x^3 \right) } \\
        f''(x) & = e^x x^4 + 8 e^x x^3 + 12 e^x x^2 \\
               & = \boxed{ e^x \left( x^4 + 8 x^3 + 12 x^2  \right) } \\
      \end{align*}

    \item[29]
      \begin{align*}
        f(x)   & = \frac{x^2}{1 + 2x} \\
        f'(x)  & = \boxed{ \frac{2x^2 + 2x}{(2x + 1)^2} } \\
        f''(x) & = \boxed{ \frac{2}{(2 x+1)^3} } \\
      \end{align*}

    \item[31]
      Find the slope:
      \begin{align*}
        y'          & = \frac{2}{(x + 1)^2} \\
        y'(1)       & = \frac{1}{2} \\
      \end{align*}

      Find the equation for the line:
      \begin{align*}
        \frac{1}{2} & = \frac{y - 1}{x - 1} \\
        y           & = \frac{x}{2} + \frac{1}{2}
      \end{align*}


    \item[32]
      Find the slope:
      \begin{align*}
        y'    & = \frac{e^x (x - 1)}{x^2} \\
        y'(1) & = 0 \\
      \end{align*}

      Find the equation for the line:
      \begin{align*}
        0 & = \frac{y - e}{x - 1} \\
        y & = e \\
      \end{align*}

    \item[33]
      Find the slope:
      \begin{align*}
        y             & = 2 x e^x \\
        y'            & = 2 e^x (x+1) \\
        y'(0)         & = 2 \\
        m_{normal}    & = - \frac{1}{2} \\
      \end{align*}

      Find the equation for the line:
      \begin{align*}
        - \frac{1}{2} & = \frac{y - e}{x - 1} \\
        y             & = - \frac{x}{2} \\
      \end{align*}

    \item[41]
      \begin{align*}
        f(x)   & = \frac{x^2}{1 + x} \\
        f'(x)  & = \frac{x^2 + 2x}{(x + 1)^2} \\
               & = \frac{x^2 + 2x}{x^2 + 2x + 1} \\
        f''(x) & = \frac{(2x + 2)(x + 1)^2 - \left( x^2 + 2x \right)(2x + 2)}{(x + 1)^4} \\
               & = \frac{(2x + 2)(x + 1)^2 - 2 \left( x^2 + 2x \right)(x + 1)}{(x + 1)^4} \\
               & = \frac{(2x + 2)(x + 1) - 2 \left( x^2 + 2x \right)}{(x + 1)^3} \\
               & = \frac{2}{(x + 1)^3} \\
        f''(1) & = \boxed{ \frac{1}{4} } \\
      \end{align*}

    \newpage

    \item[43]
      \begin{enumerate}[(a)]

        \item 
          \[
            (fg)'(5) = f(5)g'(5) + g(5)f'(5) = \boxed{ -16 }
          \]

        \item 
          \[
            \left( \frac{f}{g} \right)'(5) = \frac{f(5)g'(5) - g(5)f'(5)}{g(5)^2} 
              = \boxed{ - \frac{20}{9} }
          \]

        \item 
          \[
            \left( \frac{g}{f} \right)'(5) = \frac{g(5)f'(5) - f(5)g'(5)}{f(5)^2} = \boxed{ 20 }
          \]

      \end{enumerate}

    \item[45]
      \begin{align*}
        f(x)  & = e^x g(x) \\
        f'(x) & = e^x g(x) + e^x g'(x) \\
              & = e^x (g(x) + g'(x)) \\
        f'(0) & = e^0 ( 2 + 5 ) \\
              & = \boxed{ 7 } \\
      \end{align*}

    \item[49]
      \begin{enumerate}[(a)]

        \item 
          \begin{align*}
            y  & = x g(x) \\
            y' & = \boxed{ x g'(x) + g(x) } \\
          \end{align*}

        \item 
          \begin{align*}
            y  & = \frac{x}{g(x)} \\
            y' & = \boxed{ \frac{g(x) - x g'(x)}{[g(x)]^2} } \\
          \end{align*}

        \item 
          \begin{align*}
            y  & = \frac{g(x)}{x} \\
            y' & = \boxed{ \frac{x g'(x) - g(x)}{x^2} } \\
          \end{align*}

      \end{enumerate}

    \item[58]
      \begin{enumerate}[(a)]
        \item 
          \begin{align*}
            \frac{d}{dx} \left[ \frac{1}{g(x)} \right] & = \frac{0 - g'(x)}{[g(x)]^2} \\
                                                       & = \boxed{ - \frac{g'(x)}{[g(x)]^2} } \\
          \end{align*}

        \item 
          \begin{align*}
            y  & = \frac{1}{s + k e^s} \\
            y' & = - \frac{1 + k e^s}{ \left( s + k e^s \right)^2} \\
               & = \boxed{ \frac{-1 - k e^s}{ \left( s + k e^s \right)^2} } \\
          \end{align*}

        \item
          \begin{align*}
            \frac{d}{dx} \left( x^{-n} \right) 
              & = \frac{d}{dx} \left( \frac{1}{x^n} \right) \\
              & = \frac{- n x^{n - 1}}{x^{2n}} \\
              & = - n x^{-n - 1} \\
          \end{align*}
      \end{enumerate}

   \end{description}
 
  \else
    \vspace{10 cm}
    \begin{quote}
      \begin{em}
        The ideally non-violent state will be an ordered anarchy. That state is
        the best governed which is governed the least.
      \end{em}
    \end{quote}
    \hspace{2 cm} --Mahatma Gandhi
  \fi

\end{document}

